wip

proofs/fstar/extraction-edited/Libcrux.Kem.Kyber.Ind_cpa.fst
@@ -1,42 +1,97 @@
 module Libcrux.Kem.Kyber.Ind_cpa
-#set-options "--fuel 0 --ifuel 1 --z3rlimit 100"
+#set-options "--fuel 0 --ifuel 1 --z3rlimit 15"
 open Core
 open FStar.Mul
 
-let serialize_secret_key
-      (v_SERIALIZED_KEY_LEN: usize)
-      (private_key public_key implicit_rejection_value: t_Slice u8) =
-  let res = 
-  Libcrux.Kem.Kyber.Conversions.impl__array v_SERIALIZED_KEY_LEN
-    (Libcrux.Kem.Kyber.Conversions.f_push (Libcrux.Kem.Kyber.Conversions.f_push (Libcrux.Kem.Kyber.Conversions.f_push
-                (Libcrux.Kem.Kyber.Conversions.f_push (Libcrux.Kem.Kyber.Conversions.impl__new v_SERIALIZED_KEY_LEN
-                        (Rust_primitives.Hax.repeat 0uy v_SERIALIZED_KEY_LEN
-                          <:
-                          t_Array u8 v_SERIALIZED_KEY_LEN)
-                      <:
-                      Libcrux.Kem.Kyber.Conversions.t_UpdatableArray v_SERIALIZED_KEY_LEN)
-                    private_key
-                  <:
-                  Libcrux.Kem.Kyber.Conversions.t_UpdatableArray v_SERIALIZED_KEY_LEN)
-                public_key
+let into_padded_array (v_LEN: usize) (slice: t_Slice u8) =
+  let _:Prims.unit =
+    if true
+    then
+      let _:Prims.unit =
+        if ~.((Core.Slice.impl__len slice <: usize) <=. v_LEN <: bool)
+        then
+          Rust_primitives.Hax.never_to_any (Core.Panicking.panic "assertion failed: slice.len() <= LEN"
+
               <:
-              Libcrux.Kem.Kyber.Conversions.t_UpdatableArray v_SERIALIZED_KEY_LEN)
-            (Rust_primitives.unsize (Libcrux.Kem.Kyber.Hash_functions.v_H public_key
-                  <:
-                  t_Array u8 (sz 32))
+              Rust_primitives.Hax.t_Never)
+      in
+      ()
+  in
+  let out:t_Array u8 v_LEN = Rust_primitives.Hax.repeat 0uy v_LEN in
+  let out:t_Array u8 v_LEN =
+    Rust_primitives.Hax.Monomorphized_update_at.update_at_range out
+      ({ Core.Ops.Range.f_start = sz 0; Core.Ops.Range.f_end = Core.Slice.impl__len slice <: usize }
+        <:
+        Core.Ops.Range.t_Range usize)
+      (Core.Slice.impl__copy_from_slice (out.[ {
+                Core.Ops.Range.f_start = sz 0;
+                Core.Ops.Range.f_end = Core.Slice.impl__len slice <: usize
+              }
               <:
-              t_Slice u8)
-          <:
-          Libcrux.Kem.Kyber.Conversions.t_UpdatableArray v_SERIALIZED_KEY_LEN)
-        implicit_rejection_value
-      <:
-      Libcrux.Kem.Kyber.Conversions.t_UpdatableArray v_SERIALIZED_KEY_LEN)
-   in
-   admit(); // P-F Done, F-C Assumed
-   res
+              Core.Ops.Range.t_Range usize ]
+            <:
+            t_Slice u8)
+          slice
+        <:
+        t_Slice u8)
+  in
+  out
 
 unfold let acc_t v_K = (u8 & t_Array u8 (sz 33) & t_Array Libcrux.Kem.Kyber.Arithmetic.t_PolynomialRingElement v_K)
 unfold let inv_t v_K = acc_t v_K -> usize -> Type
+
+let sample_ring_element_cbd
+      (v_K v_ETA2_RANDOMNESS_SIZE v_ETA2: usize)
+      (prf_input: t_Array u8 (sz 33))
+      (domain_separator: u8{v domain_separator <= v v_K /\ v_K <=. sz 4})
+    : (t_Array u8 (sz 33) & u8 & t_Array Libcrux.Kem.Kyber.Arithmetic.t_PolynomialRingElement v_K) =
+  let error_1_:t_Array Libcrux.Kem.Kyber.Arithmetic.t_PolynomialRingElement v_K =
+    Rust_primitives.Hax.repeat Libcrux.Kem.Kyber.Arithmetic.impl__PolynomialRingElement__ZERO v_K
+  in
+  let orig_domain_separator = domain_separator in
+  [@ inline_let]
+  let inv : inv_t v_K = fun (acc:acc_t v_K) (i:usize) ->
+    let (domain_separator,prf_input,error_1_) = acc in
+    if (i >=. sz 0 && i <=. v_K)
+    then 
+      domain_separator = orig_domain_separator +! (mk_int #u8_inttype (v i))
+    else true in
+  let (domain_separator, prf_input, error_1_):acc_t v_K = 
+    Rust_primitives.Iterators.foldi_range #_ #(acc_t v_K)  #inv {
+              Core.Ops.Range.f_start = sz 0;
+              Core.Ops.Range.f_end = v_K
+            }
+      (domain_separator, prf_input, error_1_)
+      (fun temp_0_ i ->
+          let domain_separator, prf_input, error_1_:acc_t v_K =
+            temp_0_
+          in
+          let i:usize = i in
+          let prf_input:t_Array u8 (sz 33) =
+            Rust_primitives.Hax.Monomorphized_update_at.update_at_usize prf_input
+              (sz 32)
+              domain_separator
+          in
+          let domain_separator:u8 = domain_separator +! 1uy in
+          let (prf_output: t_Array u8 v_ETA2_RANDOMNESS_SIZE):t_Array u8 v_ETA2_RANDOMNESS_SIZE =
+            Libcrux.Kem.Kyber.Hash_functions.v_PRF v_ETA2_RANDOMNESS_SIZE
+              (Rust_primitives.unsize prf_input <: t_Slice u8)
+          in
+          let error_1_:t_Array Libcrux.Kem.Kyber.Arithmetic.t_PolynomialRingElement v_K =
+            Rust_primitives.Hax.Monomorphized_update_at.update_at_usize error_1_
+              i
+              (Libcrux.Kem.Kyber.Sampling.sample_from_binomial_distribution v_ETA2
+                  (Rust_primitives.unsize prf_output <: t_Slice u8)
+                <:
+                Libcrux.Kem.Kyber.Arithmetic.t_PolynomialRingElement)
+          in
+          domain_separator, prf_input, error_1_)
+  in
+  let hax_temp_output:t_Array Libcrux.Kem.Kyber.Arithmetic.t_PolynomialRingElement v_K = error_1_ in
+  prf_input, domain_separator, hax_temp_output
+  <:
+  (t_Array u8 (sz 33) & u8 & t_Array Libcrux.Kem.Kyber.Arithmetic.t_PolynomialRingElement v_K)
+
 let sample_vector_cbd_then_ntt
       (v_K v_ETA v_ETA_RANDOMNESS_SIZE: usize)
       (prf_input: t_Array u8 (sz 33))
@@ -98,164 +153,13 @@ let sample_vector_cbd_then_ntt
   <:
   (t_Array Libcrux.Kem.Kyber.Arithmetic.t_PolynomialRingElement v_K & u8)
 
-let sample_matrix_A (v_K: usize) (seed: t_Array u8 (sz 34)) (transpose: bool)
-    : (t_Array (t_Array Libcrux.Kem.Kyber.Arithmetic.t_PolynomialRingElement v_K) v_K &
-      Core.Option.t_Option Libcrux.Kem.Kyber.Types.t_Error) =
-  let v_A_transpose:t_Array (t_Array Libcrux.Kem.Kyber.Arithmetic.t_PolynomialRingElement v_K) v_K =
-    Rust_primitives.Hax.repeat (Rust_primitives.Hax.repeat Libcrux.Kem.Kyber.Arithmetic.impl__PolynomialRingElement__ZERO
-          v_K
-        <:
-        t_Array Libcrux.Kem.Kyber.Arithmetic.t_PolynomialRingElement v_K)
-      v_K
-  in
-  let sampling_A_error:Core.Option.t_Option Libcrux.Kem.Kyber.Types.t_Error =
-    Core.Option.Option_None <: Core.Option.t_Option Libcrux.Kem.Kyber.Types.t_Error
-  in
-  let v_A_transpose, sampling_A_error:(t_Array
-      (t_Array Libcrux.Kem.Kyber.Arithmetic.t_PolynomialRingElement v_K) v_K &
-    Core.Option.t_Option Libcrux.Kem.Kyber.Types.t_Error) =
-    Core.Iter.Traits.Iterator.f_fold (Core.Iter.Traits.Collect.f_into_iter ({
-              Core.Ops.Range.f_start = sz 0;
-              Core.Ops.Range.f_end = v_K
-            }
-            <:
-            Core.Ops.Range.t_Range usize)
-        <:
-        Core.Ops.Range.t_Range usize)
-      (v_A_transpose, sampling_A_error
-        <:
-        (t_Array (t_Array Libcrux.Kem.Kyber.Arithmetic.t_PolynomialRingElement v_K) v_K &
-          Core.Option.t_Option Libcrux.Kem.Kyber.Types.t_Error))
-      (fun temp_0_ i ->
-          let v_A_transpose, sampling_A_error:(t_Array
-              (t_Array Libcrux.Kem.Kyber.Arithmetic.t_PolynomialRingElement v_K) v_K &
-            Core.Option.t_Option Libcrux.Kem.Kyber.Types.t_Error) =
-            temp_0_
-          in
-          let i:usize = i in
-          let seeds:t_Array (t_Array u8 (sz 34)) v_K = Rust_primitives.Hax.repeat seed v_K in
-          let seeds:t_Array (t_Array u8 (sz 34)) v_K =
-            Core.Iter.Traits.Iterator.f_fold (Core.Iter.Traits.Collect.f_into_iter ({
-                      Core.Ops.Range.f_start = sz 0;
-                      Core.Ops.Range.f_end = v_K
-                    }
-                    <:
-                    Core.Ops.Range.t_Range usize)
-                <:
-                Core.Ops.Range.t_Range usize)
-              seeds
-              (fun seeds j ->
-                  let seeds:t_Array (t_Array u8 (sz 34)) v_K = seeds in
-                  let j:usize = j in
-                  let seeds:t_Array (t_Array u8 (sz 34)) v_K =
-                    Rust_primitives.Hax.Monomorphized_update_at.update_at_usize seeds
-                      j
-                      (Rust_primitives.Hax.Monomorphized_update_at.update_at_usize (seeds.[ j ]
-                            <:
-                            t_Array u8 (sz 34))
-                          (sz 32)
-                          (cast (i <: usize) <: u8)
-                        <:
-                        t_Array u8 (sz 34))
-                  in
-                  let seeds:t_Array (t_Array u8 (sz 34)) v_K =
-                    Rust_primitives.Hax.Monomorphized_update_at.update_at_usize seeds
-                      j
-                      (Rust_primitives.Hax.Monomorphized_update_at.update_at_usize (seeds.[ j ]
-                            <:
-                            t_Array u8 (sz 34))
-                          (sz 33)
-                          (cast (j <: usize) <: u8)
-                        <:
-                        t_Array u8 (sz 34))
-                  in
-                  seeds)
-          in
-          let xof_bytes:t_Array (t_Array u8 (sz 840)) v_K =
-            Libcrux.Kem.Kyber.Hash_functions.v_XOFx4 (sz 840) v_K seeds
-          in
-          Core.Iter.Traits.Iterator.f_fold (Core.Iter.Traits.Collect.f_into_iter ({
-                    Core.Ops.Range.f_start = sz 0;
-                    Core.Ops.Range.f_end = v_K
-                  }
-                  <:
-                  Core.Ops.Range.t_Range usize)
-              <:
-              Core.Ops.Range.t_Range usize)
-            (v_A_transpose, sampling_A_error
-              <:
-              (t_Array (t_Array Libcrux.Kem.Kyber.Arithmetic.t_PolynomialRingElement v_K) v_K &
-                Core.Option.t_Option Libcrux.Kem.Kyber.Types.t_Error))
-            (fun temp_0_ j ->
-                let v_A_transpose, sampling_A_error:(t_Array
-                    (t_Array Libcrux.Kem.Kyber.Arithmetic.t_PolynomialRingElement v_K) v_K &
-                  Core.Option.t_Option Libcrux.Kem.Kyber.Types.t_Error) =
-                  temp_0_
-                in
-                let j:usize = j in
-                let sampled, error:(Libcrux.Kem.Kyber.Arithmetic.t_PolynomialRingElement &
-                  Core.Option.t_Option Libcrux.Kem.Kyber.Types.t_Error) =
-                  Libcrux.Kem.Kyber.Sampling.sample_from_uniform_distribution (sz 840)
-                    (xof_bytes.[ j ] <: t_Array u8 (sz 840))
-                in
-                let sampling_A_error:Core.Option.t_Option Libcrux.Kem.Kyber.Types.t_Error =
-                  if Core.Option.impl__is_some error
-                  then
-                    let sampling_A_error:Core.Option.t_Option Libcrux.Kem.Kyber.Types.t_Error =
-                      error
-                    in
-                    sampling_A_error
-                  else sampling_A_error
-                in
-                if transpose
-                then
-                  let v_A_transpose:t_Array
-                    (t_Array Libcrux.Kem.Kyber.Arithmetic.t_PolynomialRingElement v_K) v_K =
-                    Rust_primitives.Hax.Monomorphized_update_at.update_at_usize v_A_transpose
-                      j
-                      (Rust_primitives.Hax.Monomorphized_update_at.update_at_usize (v_A_transpose.[ j
-                            ]
-                            <:
-                            t_Array Libcrux.Kem.Kyber.Arithmetic.t_PolynomialRingElement v_K)
-                          i
-                          sampled
-                        <:
-                        t_Array Libcrux.Kem.Kyber.Arithmetic.t_PolynomialRingElement v_K)
-                  in
-                  v_A_transpose, sampling_A_error
-                  <:
-                  (t_Array (t_Array Libcrux.Kem.Kyber.Arithmetic.t_PolynomialRingElement v_K) v_K &
-                    Core.Option.t_Option Libcrux.Kem.Kyber.Types.t_Error)
-                else
-                  let v_A_transpose:t_Array
-                    (t_Array Libcrux.Kem.Kyber.Arithmetic.t_PolynomialRingElement v_K) v_K =
-                    Rust_primitives.Hax.Monomorphized_update_at.update_at_usize v_A_transpose
-                      i
-                      (Rust_primitives.Hax.Monomorphized_update_at.update_at_usize (v_A_transpose.[ i
-                            ]
-                            <:
-                            t_Array Libcrux.Kem.Kyber.Arithmetic.t_PolynomialRingElement v_K)
-                          j
-                          sampled
-                        <:
-                        t_Array Libcrux.Kem.Kyber.Arithmetic.t_PolynomialRingElement v_K)
-                  in
-                  v_A_transpose, sampling_A_error
-                  <:
-                  (t_Array (t_Array Libcrux.Kem.Kyber.Arithmetic.t_PolynomialRingElement v_K) v_K &
-                    Core.Option.t_Option Libcrux.Kem.Kyber.Types.t_Error)))
-  in
-  v_A_transpose, sampling_A_error
-  <:
-  (t_Array (t_Array Libcrux.Kem.Kyber.Arithmetic.t_PolynomialRingElement v_K) v_K &
-    Core.Option.t_Option Libcrux.Kem.Kyber.Types.t_Error)
-
-let compress_then_encode_u
+let compress_then_serialize_u
       (v_K v_OUT_LEN v_COMPRESSION_FACTOR v_BLOCK_LEN: usize)
       (input: t_Array Libcrux.Kem.Kyber.Arithmetic.t_PolynomialRingElement v_K)
     : Pure (t_Array u8 v_OUT_LEN)
       (requires (v_K >. sz 0)) 
       (ensures (fun _ -> True)) =
+  admit();
   let out:t_Array u8 v_OUT_LEN = Rust_primitives.Hax.repeat 0uy v_OUT_LEN in
   let out:t_Array u8 v_OUT_LEN =
     Core.Iter.Traits.Iterator.f_fold (Core.Iter.Traits.Collect.f_into_iter (Core.Iter.Traits.Iterator.f_enumerate
@@ -274,6 +178,7 @@ let compress_then_encode_u
           let i, re:(usize & Libcrux.Kem.Kyber.Arithmetic.t_PolynomialRingElement) = temp_1_ in
           assume ((v i + 1) < v v_OUT_LEN);
           assume (((v i + 1) * (v v_OUT_LEN / v v_K)) < v v_OUT_LEN);
+          
           Rust_primitives.Hax.Monomorphized_update_at.update_at_range out
             ({
                 Core.Ops.Range.f_start = i *! (v_OUT_LEN /! v_K <: usize) <: usize;
@@ -306,7 +211,239 @@ let compress_then_encode_u
   in
   out
 
-let serialize_key
+let deserialize_then_decompress_u #p
+      (v_K v_CIPHERTEXT_SIZE v_VECTOR_U_ENCODED_SIZE v_U_COMPRESSION_FACTOR: usize)
+      (ciphertext: t_Array u8 v_CIPHERTEXT_SIZE)
+    : t_Array Libcrux.Kem.Kyber.Arithmetic.t_PolynomialRingElement v_K =
+  let u_as_ntt:t_Array Libcrux.Kem.Kyber.Arithmetic.t_PolynomialRingElement v_K =
+    Rust_primitives.Hax.repeat Libcrux.Kem.Kyber.Arithmetic.impl__PolynomialRingElement__ZERO v_K
+  in
+  let acc_t1 = t_Array Libcrux.Kem.Kyber.Arithmetic.t_PolynomialRingElement v_K in
+  [@ inline_let]
+  let inv = fun (acc:acc_t1) (i:usize) -> True in
+  let sl : t_Slice u8 = ciphertext.Libcrux.Kem.Kyber.Types.f_value.[ 
+                      { Core.Ops.Range.f_end = v_VECTOR_U_ENCODED_SIZE  } <: Core.Ops.Range.t_RangeTo usize ] in
+  assert (length sl == v_VECTOR_U_ENCODED_SIZE);
+  let chunk_len = ((Libcrux.Kem.Kyber.Constants.v_COEFFICIENTS_IN_RING_ELEMENT *!
+                      v_U_COMPRESSION_FACTOR
+                      <:
+                      usize) /!
+                    sz 8
+                    <:
+                    usize) in
+  assert (v chunk_len == (256 * v v_U_COMPRESSION_FACTOR) / 8);
+  assert (chunk_len == Spec.Kyber.v_C1_BLOCK_SIZE p);
+  assert (length sl == Spec.Kyber.v_C1_SIZE p);
+  assert (Seq.length sl % v chunk_len == 0);
+  admit();
+  let u_as_ntt:t_Array Libcrux.Kem.Kyber.Arithmetic.t_PolynomialRingElement v_K =
+   Rust_primitives.Iterators.foldi_chunks_exact #u8 #acc_t1 #inv
+      sl
+      chunk_len
+      u_as_ntt
+      (fun u_as_ntt temp_1_ ->
+          let u_as_ntt:t_Array Libcrux.Kem.Kyber.Arithmetic.t_PolynomialRingElement v_K =
+            u_as_ntt
+          in
+          let i, u_bytes:(usize & t_Slice u8) = temp_1_ in
+          let u:Libcrux.Kem.Kyber.Arithmetic.t_PolynomialRingElement =
+            Libcrux.Kem.Kyber.Serialize.deserialize_then_decompress_ring_element_u v_U_COMPRESSION_FACTOR
+              u_bytes
+          in
+          let u_as_ntt:t_Array Libcrux.Kem.Kyber.Arithmetic.t_PolynomialRingElement v_K =
+            Rust_primitives.Hax.Monomorphized_update_at.update_at_usize u_as_ntt
+              i
+              (Libcrux.Kem.Kyber.Ntt.ntt_vector_u v_U_COMPRESSION_FACTOR u
+                <:
+                Libcrux.Kem.Kyber.Arithmetic.t_PolynomialRingElement)
+          in
+          u_as_ntt)
+  in
+  u_as_ntt
+
+let deserialize_public_key (v_K v_T_AS_NTT_ENCODED_SIZE: usize) (public_key: t_Slice u8)
+    : t_Array Libcrux.Kem.Kyber.Arithmetic.t_PolynomialRingElement v_K =
+  let tt_as_ntt:t_Array Libcrux.Kem.Kyber.Arithmetic.t_PolynomialRingElement v_K =
+    Rust_primitives.Hax.repeat Libcrux.Kem.Kyber.Arithmetic.impl__PolynomialRingElement__ZERO v_K
+  in
+  let tt_as_ntt:t_Array Libcrux.Kem.Kyber.Arithmetic.t_PolynomialRingElement v_K =
+    Core.Iter.Traits.Iterator.f_fold (Core.Iter.Traits.Collect.f_into_iter (Core.Iter.Traits.Iterator.f_enumerate
+              (Core.Slice.impl__chunks_exact (public_key.[ {
+                        Core.Ops.Range.f_end = v_T_AS_NTT_ENCODED_SIZE
+                      }
+                      <:
+                      Core.Ops.Range.t_RangeTo usize ]
+                    <:
+                    t_Slice u8)
+                  Libcrux.Kem.Kyber.Constants.v_BYTES_PER_RING_ELEMENT
+                <:
+                Core.Slice.Iter.t_ChunksExact u8)
+            <:
+            Core.Iter.Adapters.Enumerate.t_Enumerate (Core.Slice.Iter.t_ChunksExact u8))
+        <:
+        Core.Iter.Adapters.Enumerate.t_Enumerate (Core.Slice.Iter.t_ChunksExact u8))
+      tt_as_ntt
+      (fun tt_as_ntt temp_1_ ->
+          let tt_as_ntt:t_Array Libcrux.Kem.Kyber.Arithmetic.t_PolynomialRingElement v_K =
+            tt_as_ntt
+          in
+          let i, tt_as_ntt_bytes:(usize & t_Slice u8) = temp_1_ in
+          Rust_primitives.Hax.Monomorphized_update_at.update_at_usize tt_as_ntt
+            i
+            (Libcrux.Kem.Kyber.Serialize.deserialize_to_uncompressed_ring_element tt_as_ntt_bytes
+              <:
+              Libcrux.Kem.Kyber.Arithmetic.t_PolynomialRingElement)
+          <:
+          t_Array Libcrux.Kem.Kyber.Arithmetic.t_PolynomialRingElement v_K)
+  in
+  tt_as_ntt
+
+let deserialize_secret_key (v_K: usize) (secret_key: t_Slice u8)
+    : t_Array Libcrux.Kem.Kyber.Arithmetic.t_PolynomialRingElement v_K =
+  let secret_as_ntt:t_Array Libcrux.Kem.Kyber.Arithmetic.t_PolynomialRingElement v_K =
+    Rust_primitives.Hax.repeat Libcrux.Kem.Kyber.Arithmetic.impl__PolynomialRingElement__ZERO v_K
+  in
+  let secret_as_ntt:t_Array Libcrux.Kem.Kyber.Arithmetic.t_PolynomialRingElement v_K =
+    Core.Iter.Traits.Iterator.f_fold (Core.Iter.Traits.Collect.f_into_iter (Core.Iter.Traits.Iterator.f_enumerate
+              (Core.Slice.impl__chunks_exact secret_key
+                  Libcrux.Kem.Kyber.Constants.v_BYTES_PER_RING_ELEMENT
+                <:
+                Core.Slice.Iter.t_ChunksExact u8)
+            <:
+            Core.Iter.Adapters.Enumerate.t_Enumerate (Core.Slice.Iter.t_ChunksExact u8))
+        <:
+        Core.Iter.Adapters.Enumerate.t_Enumerate (Core.Slice.Iter.t_ChunksExact u8))
+      secret_as_ntt
+      (fun secret_as_ntt temp_1_ ->
+          let secret_as_ntt:t_Array Libcrux.Kem.Kyber.Arithmetic.t_PolynomialRingElement v_K =
+            secret_as_ntt
+          in
+          let i, secret_bytes:(usize & t_Slice u8) = temp_1_ in
+          Rust_primitives.Hax.Monomorphized_update_at.update_at_usize secret_as_ntt
+            i
+            (Libcrux.Kem.Kyber.Serialize.deserialize_to_uncompressed_ring_element secret_bytes
+              <:
+              Libcrux.Kem.Kyber.Arithmetic.t_PolynomialRingElement)
+          <:
+          t_Array Libcrux.Kem.Kyber.Arithmetic.t_PolynomialRingElement v_K)
+  in
+  secret_as_ntt
+
+let decrypt
+      (v_K v_CIPHERTEXT_SIZE v_VECTOR_U_ENCODED_SIZE v_U_COMPRESSION_FACTOR v_V_COMPRESSION_FACTOR:
+          usize)
+      (secret_key: t_Slice u8)
+      (ciphertext: t_Array u8 v_CIPHERTEXT_SIZE)
+    : t_Array u8 (sz 32) =
+  let u_as_ntt:t_Array Libcrux.Kem.Kyber.Arithmetic.t_PolynomialRingElement v_K =
+    deserialize_then_decompress_u v_K
+      v_CIPHERTEXT_SIZE
+      v_VECTOR_U_ENCODED_SIZE
+      v_U_COMPRESSION_FACTOR
+      ciphertext
+  in
+  let v:Libcrux.Kem.Kyber.Arithmetic.t_PolynomialRingElement =
+    Libcrux.Kem.Kyber.Serialize.deserialize_then_decompress_ring_element_v v_V_COMPRESSION_FACTOR
+      (ciphertext.[ { Core.Ops.Range.f_start = v_VECTOR_U_ENCODED_SIZE }
+          <:
+          Core.Ops.Range.t_RangeFrom usize ]
+        <:
+        t_Slice u8)
+  in
+  let secret_as_ntt:t_Array Libcrux.Kem.Kyber.Arithmetic.t_PolynomialRingElement v_K =
+    deserialize_secret_key v_K secret_key
+  in
+  let message:Libcrux.Kem.Kyber.Arithmetic.t_PolynomialRingElement =
+    Libcrux.Kem.Kyber.Matrix.compute_message v_K v secret_as_ntt u_as_ntt
+  in
+  Libcrux.Kem.Kyber.Serialize.compress_then_serialize_message message
+
+let encrypt
+      (v_K v_CIPHERTEXT_SIZE v_T_AS_NTT_ENCODED_SIZE v_C1_LEN v_C2_LEN v_U_COMPRESSION_FACTOR v_V_COMPRESSION_FACTOR v_BLOCK_LEN v_ETA1 v_ETA1_RANDOMNESS_SIZE v_ETA2 v_ETA2_RANDOMNESS_SIZE:
+          usize)
+      (public_key: t_Slice u8)
+      (message: t_Array u8 (sz 32))
+      (randomness: t_Slice u8)
+    : (t_Array u8 v_CIPHERTEXT_SIZE & Core.Option.t_Option Libcrux.Kem.Kyber.Types.t_Error) =
+  let tt_as_ntt:t_Array Libcrux.Kem.Kyber.Arithmetic.t_PolynomialRingElement v_K =
+    deserialize_public_key v_K v_T_AS_NTT_ENCODED_SIZE public_key
+  in
+  let seed:t_Slice u8 =
+    public_key.[ { Core.Ops.Range.f_start = v_T_AS_NTT_ENCODED_SIZE }
+      <:
+      Core.Ops.Range.t_RangeFrom usize ]
+  in
+  let v_A_transpose, sampling_A_error:(t_Array
+      (t_Array Libcrux.Kem.Kyber.Arithmetic.t_PolynomialRingElement v_K) v_K &
+    Core.Option.t_Option Libcrux.Kem.Kyber.Types.t_Error) =
+    Libcrux.Kem.Kyber.Matrix.sample_matrix_A v_K
+      (into_padded_array (sz 34) seed <: t_Array u8 (sz 34))
+      false
+  in
+  let (prf_input: t_Array u8 (sz 33)):t_Array u8 (sz 33) = into_padded_array (sz 33) randomness in
+  let r_as_ntt, domain_separator:(t_Array Libcrux.Kem.Kyber.Arithmetic.t_PolynomialRingElement v_K &
+    u8) =
+    sample_vector_cbd_then_ntt v_K v_ETA1 v_ETA1_RANDOMNESS_SIZE prf_input 0uy
+  in
+  let tmp0, tmp1, out:(t_Array u8 (sz 33) & u8 &
+    t_Array Libcrux.Kem.Kyber.Arithmetic.t_PolynomialRingElement v_K) =
+    sample_ring_element_cbd v_K v_ETA2_RANDOMNESS_SIZE v_ETA2 prf_input domain_separator
+  in
+  let prf_input:t_Array u8 (sz 33) = tmp0 in
+  let domain_separator:u8 = tmp1 in
+  let error_1_:t_Array Libcrux.Kem.Kyber.Arithmetic.t_PolynomialRingElement v_K = out in
+  let prf_input:t_Array u8 (sz 33) =
+    Rust_primitives.Hax.Monomorphized_update_at.update_at_usize prf_input (sz 32) domain_separator
+  in
+  let (prf_output: t_Array u8 v_ETA2_RANDOMNESS_SIZE):t_Array u8 v_ETA2_RANDOMNESS_SIZE =
+    Libcrux.Kem.Kyber.Hash_functions.v_PRF v_ETA2_RANDOMNESS_SIZE
+      (Rust_primitives.unsize prf_input <: t_Slice u8)
+  in
+  let error_2_:Libcrux.Kem.Kyber.Arithmetic.t_PolynomialRingElement =
+    Libcrux.Kem.Kyber.Sampling.sample_from_binomial_distribution v_ETA2
+      (Rust_primitives.unsize prf_output <: t_Slice u8)
+  in
+  let u:t_Array Libcrux.Kem.Kyber.Arithmetic.t_PolynomialRingElement v_K =
+    Libcrux.Kem.Kyber.Matrix.compute_vector_u v_K v_A_transpose r_as_ntt error_1_
+  in
+  let message_as_ring_element:Libcrux.Kem.Kyber.Arithmetic.t_PolynomialRingElement =
+    Libcrux.Kem.Kyber.Serialize.deserialize_then_decompress_message message
+  in
+  let v:Libcrux.Kem.Kyber.Arithmetic.t_PolynomialRingElement =
+    Libcrux.Kem.Kyber.Matrix.compute_ring_element_v v_K
+      tt_as_ntt
+      r_as_ntt
+      error_2_
+      message_as_ring_element
+  in
+  let c1:t_Array u8 v_C1_LEN =
+    compress_then_serialize_u v_K v_C1_LEN v_U_COMPRESSION_FACTOR v_BLOCK_LEN u
+  in
+  let c2:t_Array u8 v_C2_LEN =
+    Libcrux.Kem.Kyber.Serialize.compress_then_serialize_ring_element_v v_V_COMPRESSION_FACTOR
+      v_C2_LEN
+      v
+  in
+  let (ciphertext: t_Array u8 v_CIPHERTEXT_SIZE):t_Array u8 v_CIPHERTEXT_SIZE =
+    into_padded_array v_CIPHERTEXT_SIZE (Rust_primitives.unsize c1 <: t_Slice u8)
+  in
+  let ciphertext:t_Array u8 v_CIPHERTEXT_SIZE =
+    Rust_primitives.Hax.Monomorphized_update_at.update_at_range_from ciphertext
+      ({ Core.Ops.Range.f_start = v_C1_LEN } <: Core.Ops.Range.t_RangeFrom usize)
+      (Core.Slice.impl__copy_from_slice (ciphertext.[ { Core.Ops.Range.f_start = v_C1_LEN }
+              <:
+              Core.Ops.Range.t_RangeFrom usize ]
+            <:
+            t_Slice u8)
+          (Core.Array.impl_23__as_slice v_C2_LEN c2 <: t_Slice u8)
+        <:
+        t_Slice u8)
+  in
+  ciphertext, sampling_A_error
+  <:
+  (t_Array u8 v_CIPHERTEXT_SIZE & Core.Option.t_Option Libcrux.Kem.Kyber.Types.t_Error)
+
+let serialize_secret_key
       (v_K v_OUT_LEN: usize)
       (key: t_Array Libcrux.Kem.Kyber.Arithmetic.t_PolynomialRingElement v_K)
     : t_Array u8 v_OUT_LEN =
@@ -326,8 +463,6 @@ let serialize_key
       (fun out temp_1_ ->
           let out:t_Array u8 v_OUT_LEN = out in
           let i, re:(usize & Libcrux.Kem.Kyber.Arithmetic.t_PolynomialRingElement) = temp_1_ in
-
-          assume ((v i + 1) * v Libcrux.Kem.Kyber.Constants.v_BYTES_PER_RING_ELEMENT < v v_OUT_LEN);          
           Rust_primitives.Hax.Monomorphized_update_at.update_at_range out
             ({
                 Core.Ops.Range.f_start
@@ -368,248 +503,61 @@ let serialize_key
   in
   out
 
-let decrypt
-      (v_K v_CIPHERTEXT_SIZE v_VECTOR_U_ENCODED_SIZE v_U_COMPRESSION_FACTOR v_V_COMPRESSION_FACTOR:
-          usize)
-      (secret_key: t_Slice u8)
-      (ciphertext: Libcrux.Kem.Kyber.Types.t_KyberCiphertext v_CIPHERTEXT_SIZE) =
-  let u_as_ntt:t_Array Libcrux.Kem.Kyber.Arithmetic.t_PolynomialRingElement v_K =
-    Rust_primitives.Hax.repeat Libcrux.Kem.Kyber.Arithmetic.impl__PolynomialRingElement__ZERO v_K
+let serialize_public_key
+      (v_K v_RANKED_BYTES_PER_RING_ELEMENT v_PUBLIC_KEY_SIZE: usize)
+      (tt_as_ntt: t_Array Libcrux.Kem.Kyber.Arithmetic.t_PolynomialRingElement v_K)
+      (seed_for_a: t_Slice u8)
+    : t_Array u8 v_PUBLIC_KEY_SIZE =
+  let public_key_serialized:t_Array u8 v_PUBLIC_KEY_SIZE =
+    Rust_primitives.Hax.repeat 0uy v_PUBLIC_KEY_SIZE
   in
-  let secret_as_ntt:t_Array Libcrux.Kem.Kyber.Arithmetic.t_PolynomialRingElement v_K =
-    Rust_primitives.Hax.repeat Libcrux.Kem.Kyber.Arithmetic.impl__PolynomialRingElement__ZERO v_K
-  in
-  let acc_t1 = t_Array Libcrux.Kem.Kyber.Arithmetic.t_PolynomialRingElement v_K in
-  [@ inline_let]
-  let inv = fun (acc:acc_t1) (i:usize) -> True in
-  let sl : t_Slice u8 = ciphertext.Libcrux.Kem.Kyber.Types.f_value.[ 
-                      { Core.Ops.Range.f_end = v_VECTOR_U_ENCODED_SIZE  } <: Core.Ops.Range.t_RangeTo usize ] in
-  assert (length sl == v_VECTOR_U_ENCODED_SIZE);
-  let chunk_len = ((Libcrux.Kem.Kyber.Constants.v_COEFFICIENTS_IN_RING_ELEMENT *!
-                      v_U_COMPRESSION_FACTOR
-                      <:
-                      usize) /!
-                    sz 8
-                    <:
-                    usize) in
-  let u_as_ntt:t_Array Libcrux.Kem.Kyber.Arithmetic.t_PolynomialRingElement v_K =
-   Rust_primitives.Iterators.foldi_chunks_exact #u8 #acc_t1 #inv
-      sl
-      chunk_len
-      u_as_ntt
-      (fun u_as_ntt temp_1_ ->
-          let u_as_ntt:t_Array Libcrux.Kem.Kyber.Arithmetic.t_PolynomialRingElement v_K =
-            u_as_ntt
-          in
-          let i, u_bytes:(usize & t_Slice u8) = temp_1_ in
-          assert (i <. length sl /! chunk_len);
-          assert (v i < v v_K);
-          let u:Libcrux.Kem.Kyber.Arithmetic.t_PolynomialRingElement =
-            Libcrux.Kem.Kyber.Serialize.deserialize_then_decompress_ring_element_u v_U_COMPRESSION_FACTOR
-              u_bytes
-          in
-          let u_as_ntt:t_Array Libcrux.Kem.Kyber.Arithmetic.t_PolynomialRingElement v_K =
-            Rust_primitives.Hax.Monomorphized_update_at.update_at_usize u_as_ntt
-              i
-              (Libcrux.Kem.Kyber.Ntt.ntt_vector_u v_U_COMPRESSION_FACTOR u
+  let public_key_serialized:t_Array u8 v_PUBLIC_KEY_SIZE =
+    Rust_primitives.Hax.Monomorphized_update_at.update_at_range public_key_serialized
+      ({ Core.Ops.Range.f_start = sz 0; Core.Ops.Range.f_end = v_RANKED_BYTES_PER_RING_ELEMENT }
+        <:
+        Core.Ops.Range.t_Range usize)
+      (Core.Slice.impl__copy_from_slice (public_key_serialized.[ {
+                Core.Ops.Range.f_start = sz 0;
+                Core.Ops.Range.f_end = v_RANKED_BYTES_PER_RING_ELEMENT
+              }
+              <:
+              Core.Ops.Range.t_Range usize ]
+            <:
+            t_Slice u8)
+          (Rust_primitives.unsize (serialize_secret_key v_K
+                  v_RANKED_BYTES_PER_RING_ELEMENT
+                  tt_as_ntt
                 <:
-                Libcrux.Kem.Kyber.Arithmetic.t_PolynomialRingElement)
-          in
-          u_as_ntt)
-  in
-  let v:Libcrux.Kem.Kyber.Arithmetic.t_PolynomialRingElement =
-    Libcrux.Kem.Kyber.Serialize.deserialize_then_decompress_ring_element_v v_V_COMPRESSION_FACTOR
-      (ciphertext.Libcrux.Kem.Kyber.Types.f_value.[ {
-            Core.Ops.Range.f_start = v_VECTOR_U_ENCODED_SIZE
-          }
-          <:
-          Core.Ops.Range.t_RangeFrom usize ]
+                t_Array u8 v_RANKED_BYTES_PER_RING_ELEMENT)
+            <:
+            t_Slice u8)
         <:
         t_Slice u8)
   in
-  let acc_t1 = t_Array Libcrux.Kem.Kyber.Arithmetic.t_PolynomialRingElement v_K in
-  [@ inline_let]
-  let inv = fun (acc:acc_t1) (i:usize) -> True in
-  let sl : t_Slice u8 = secret_key in
-  let secret_as_ntt:t_Array Libcrux.Kem.Kyber.Arithmetic.t_PolynomialRingElement v_K =
-   Rust_primitives.Iterators.foldi_chunks_exact #u8 #acc_t1 #inv
-      sl
-      Libcrux.Kem.Kyber.Constants.v_BYTES_PER_RING_ELEMENT
-      secret_as_ntt
-      (fun secret_as_ntt temp_1_ ->
-          let secret_as_ntt:t_Array Libcrux.Kem.Kyber.Arithmetic.t_PolynomialRingElement v_K =
-            secret_as_ntt
-          in
-          let i, secret_bytes:(usize & t_Slice u8) = temp_1_ in
-          Rust_primitives.Hax.Monomorphized_update_at.update_at_usize secret_as_ntt
-            i
-            (Libcrux.Kem.Kyber.Serialize.deserialize_to_uncompressed_ring_element secret_bytes
-              <:
-              Libcrux.Kem.Kyber.Arithmetic.t_PolynomialRingElement)
-          <:
-          t_Array Libcrux.Kem.Kyber.Arithmetic.t_PolynomialRingElement v_K)
-  in
-  let message:Libcrux.Kem.Kyber.Arithmetic.t_PolynomialRingElement =
-    Libcrux.Kem.Kyber.Matrix.compute_message v_K v secret_as_ntt u_as_ntt
-  in
-  Libcrux.Kem.Kyber.Serialize.compress_then_serialize_message message
-
-let encrypt
-      (v_K v_CIPHERTEXT_SIZE v_T_AS_NTT_ENCODED_SIZE v_C1_LEN v_C2_LEN v_U_COMPRESSION_FACTOR v_V_COMPRESSION_FACTOR v_BLOCK_LEN v_ETA1 v_ETA1_RANDOMNESS_SIZE v_ETA2 v_ETA2_RANDOMNESS_SIZE:
-          usize)
-      (public_key: t_Slice u8)
-      (message: t_Array u8 (sz 32))
-      (randomness: t_Slice u8) =
-  let tt_as_ntt:t_Array Libcrux.Kem.Kyber.Arithmetic.t_PolynomialRingElement v_K =
-    Rust_primitives.Hax.repeat Libcrux.Kem.Kyber.Arithmetic.impl__PolynomialRingElement__ZERO v_K
-  in
-  let acc_t1 = t_Array Libcrux.Kem.Kyber.Arithmetic.t_PolynomialRingElement v_K in
-  [@ inline_let]
-  let inv = fun (acc:acc_t1) (i:usize) -> True in
-  let sl : t_Slice u8 = (public_key.[ {  Core.Ops.Range.f_end = v_T_AS_NTT_ENCODED_SIZE  } <: Core.Ops.Range.t_RangeTo usize]) in
-  assert (length sl == v_T_AS_NTT_ENCODED_SIZE);
-  let tt_as_ntt:t_Array Libcrux.Kem.Kyber.Arithmetic.t_PolynomialRingElement v_K =
-   Rust_primitives.Iterators.foldi_chunks_exact #u8 #acc_t1 #inv
-      sl
-      Libcrux.Kem.Kyber.Constants.v_BYTES_PER_RING_ELEMENT
-      tt_as_ntt
-      (fun tt_as_ntt temp_1_ ->
-          let tt_as_ntt:t_Array Libcrux.Kem.Kyber.Arithmetic.t_PolynomialRingElement v_K =
-            tt_as_ntt
-          in
-          let i, tt_as_ntt_bytes:(usize & t_Slice u8) = temp_1_ in
-          assert (i <. v_T_AS_NTT_ENCODED_SIZE /! Libcrux.Kem.Kyber.Constants.v_BYTES_PER_RING_ELEMENT);
-          assert (i <. v_K);
-          Rust_primitives.Hax.Monomorphized_update_at.update_at_usize tt_as_ntt
-            i
-            (Libcrux.Kem.Kyber.Serialize.deserialize_to_uncompressed_ring_element tt_as_ntt_bytes
-              <:
-              Libcrux.Kem.Kyber.Arithmetic.t_PolynomialRingElement)
-          <:
-          t_Array Libcrux.Kem.Kyber.Arithmetic.t_PolynomialRingElement v_K)
-  in
-  let seed:t_Slice u8 =
-    public_key.[ { Core.Ops.Range.f_start = v_T_AS_NTT_ENCODED_SIZE }
-      <:
-      Core.Ops.Range.t_RangeFrom usize ]
-  in
-  let v_A_transpose, sampling_A_error:(t_Array
-      (t_Array Libcrux.Kem.Kyber.Arithmetic.t_PolynomialRingElement v_K) v_K &
-    Core.Option.t_Option Libcrux.Kem.Kyber.Types.t_Error) =
-    sample_matrix_A v_K
-      (Libcrux.Kem.Kyber.Conversions.into_padded_array (sz 34) seed <: t_Array u8 (sz 34))
-      false
-  in
-  let (prf_input: t_Array u8 (sz 33)):t_Array u8 (sz 33) =
-    Libcrux.Kem.Kyber.Conversions.into_padded_array (sz 33) randomness
-  in
-  let r_as_ntt, domain_separator:(t_Array Libcrux.Kem.Kyber.Arithmetic.t_PolynomialRingElement v_K &
-    u8) =
-    sample_vector_cbd_then_ntt v_K v_ETA1 v_ETA1_RANDOMNESS_SIZE prf_input 0uy
-  in
-  let error_1_:t_Array Libcrux.Kem.Kyber.Arithmetic.t_PolynomialRingElement v_K =
-    Rust_primitives.Hax.repeat Libcrux.Kem.Kyber.Arithmetic.impl__PolynomialRingElement__ZERO v_K
-  in
-  let orig_domain_separator = domain_separator in
-  [@ inline_let]
-  let inv : inv_t v_K = fun (acc:acc_t v_K) (i:usize) ->
-    let (domain_separator,prf_input,error_1_) = acc in
-    if (i >=. sz 0 && i <=. v_K)
-    then 
-      domain_separator = orig_domain_separator +! (mk_int #u8_inttype (v i))
-    else true in
-  let (domain_separator, prf_input, error_1_):acc_t v_K = 
-    Rust_primitives.Iterators.foldi_range #_ #(acc_t v_K)  #inv {
-              Core.Ops.Range.f_start = sz 0;
-              Core.Ops.Range.f_end = v_K
-            }
-      (domain_separator, prf_input, error_1_)
-      (fun temp_0_ i ->
-          let domain_separator, prf_input, error_1_:acc_t v_K =
-            temp_0_
-          in
-          let i:usize = i in
-          let prf_input:t_Array u8 (sz 33) =
-            Rust_primitives.Hax.Monomorphized_update_at.update_at_usize prf_input
-              (sz 32)
-              domain_separator
-          in
-          let domain_separator:u8 = domain_separator +! 1uy in
-          let (prf_output: t_Array u8 v_ETA2_RANDOMNESS_SIZE):t_Array u8 v_ETA2_RANDOMNESS_SIZE =
-            Libcrux.Kem.Kyber.Hash_functions.v_PRF v_ETA2_RANDOMNESS_SIZE
-              (Rust_primitives.unsize prf_input <: t_Slice u8)
-          in
-          let error_1_:t_Array Libcrux.Kem.Kyber.Arithmetic.t_PolynomialRingElement v_K =
-            Rust_primitives.Hax.Monomorphized_update_at.update_at_usize error_1_
-              i
-              (Libcrux.Kem.Kyber.Sampling.sample_from_binomial_distribution v_ETA2
-                  (Rust_primitives.unsize prf_output <: t_Slice u8)
-                <:
-                Libcrux.Kem.Kyber.Arithmetic.t_PolynomialRingElement)
-          in
-          domain_separator, prf_input, error_1_)
-  in
-  let prf_input:t_Array u8 (sz 33) =
-    Rust_primitives.Hax.Monomorphized_update_at.update_at_usize prf_input (sz 32) domain_separator
-  in
-  let (prf_output: t_Array u8 v_ETA2_RANDOMNESS_SIZE):t_Array u8 v_ETA2_RANDOMNESS_SIZE =
-    Libcrux.Kem.Kyber.Hash_functions.v_PRF v_ETA2_RANDOMNESS_SIZE
-      (Rust_primitives.unsize prf_input <: t_Slice u8)
-  in
-  let error_2_:Libcrux.Kem.Kyber.Arithmetic.t_PolynomialRingElement =
-    Libcrux.Kem.Kyber.Sampling.sample_from_binomial_distribution v_ETA2
-      (Rust_primitives.unsize prf_output <: t_Slice u8)
-  in
-  let u:t_Array Libcrux.Kem.Kyber.Arithmetic.t_PolynomialRingElement v_K =
-    Libcrux.Kem.Kyber.Matrix.compute_vector_u v_K v_A_transpose r_as_ntt error_1_
-  in
-  let message_as_ring_element:Libcrux.Kem.Kyber.Arithmetic.t_PolynomialRingElement =
-    Libcrux.Kem.Kyber.Serialize.deserialize_then_decompress_message message
-  in
-  let v:Libcrux.Kem.Kyber.Arithmetic.t_PolynomialRingElement =
-    Libcrux.Kem.Kyber.Matrix.compute_ring_element_v v_K
-      tt_as_ntt
-      r_as_ntt
-      error_2_
-      message_as_ring_element
-  in
-  let c1:t_Array u8 v_C1_LEN =
-    compress_then_encode_u v_K v_C1_LEN v_U_COMPRESSION_FACTOR v_BLOCK_LEN u
-  in
-  let c2:t_Array u8 v_C2_LEN =
-    Libcrux.Kem.Kyber.Serialize.compress_then_serialize_ring_element_v v_V_COMPRESSION_FACTOR
-      v_C2_LEN
-      v
-  in
-  let (ciphertext: t_Array u8 v_CIPHERTEXT_SIZE):t_Array u8 v_CIPHERTEXT_SIZE =
-    Libcrux.Kem.Kyber.Conversions.into_padded_array v_CIPHERTEXT_SIZE
-      (Rust_primitives.unsize c1 <: t_Slice u8)
-  in
-  let ciphertext:t_Array u8 v_CIPHERTEXT_SIZE =
-    Rust_primitives.Hax.Monomorphized_update_at.update_at_range_from ciphertext
-      ({ Core.Ops.Range.f_start = v_C1_LEN } <: Core.Ops.Range.t_RangeFrom usize)
-      (Core.Slice.impl__copy_from_slice (ciphertext.[ { Core.Ops.Range.f_start = v_C1_LEN }
+  let public_key_serialized:t_Array u8 v_PUBLIC_KEY_SIZE =
+    Rust_primitives.Hax.Monomorphized_update_at.update_at_range_from public_key_serialized
+      ({ Core.Ops.Range.f_start = v_RANKED_BYTES_PER_RING_ELEMENT }
+        <:
+        Core.Ops.Range.t_RangeFrom usize)
+      (Core.Slice.impl__copy_from_slice (public_key_serialized.[ {
+                Core.Ops.Range.f_start = v_RANKED_BYTES_PER_RING_ELEMENT
+              }
               <:
               Core.Ops.Range.t_RangeFrom usize ]
             <:
             t_Slice u8)
-          (Core.Array.impl_23__as_slice v_C2_LEN c2 <: t_Slice u8)
+          seed_for_a
         <:
         t_Slice u8)
   in
-  let res = 
-  Core.Convert.f_into ciphertext, sampling_A_error
-  <:
-  (Libcrux.Kem.Kyber.Types.t_KyberCiphertext v_CIPHERTEXT_SIZE &
-    Core.Option.t_Option Libcrux.Kem.Kyber.Types.t_Error)
-  in
-  admit(); // P-F Done, F-C Assumed
-  res
+  public_key_serialized
 
 let generate_keypair
       (v_K v_PRIVATE_KEY_SIZE v_PUBLIC_KEY_SIZE v_RANKED_BYTES_PER_RING_ELEMENT v_ETA1 v_ETA1_RANDOMNESS_SIZE:
           usize)
-      (key_generation_seed: t_Slice u8) = 
+      (key_generation_seed: t_Slice u8)
+    : ((t_Array u8 v_PRIVATE_KEY_SIZE & t_Array u8 v_PUBLIC_KEY_SIZE) &
+      Core.Option.t_Option Libcrux.Kem.Kyber.Types.t_Error) =
   let hashed:t_Array u8 (sz 64) = Libcrux.Kem.Kyber.Hash_functions.v_G key_generation_seed in
   let seed_for_A, seed_for_secret_and_error:(t_Slice u8 & t_Slice u8) =
     Core.Slice.impl__split_at (Rust_primitives.unsize hashed <: t_Slice u8) (sz 32)
@@ -617,12 +565,12 @@ let generate_keypair
   let v_A_transpose, sampling_A_error:(t_Array
       (t_Array Libcrux.Kem.Kyber.Arithmetic.t_PolynomialRingElement v_K) v_K &
     Core.Option.t_Option Libcrux.Kem.Kyber.Types.t_Error) =
-    sample_matrix_A v_K
-      (Libcrux.Kem.Kyber.Conversions.into_padded_array (sz 34) seed_for_A <: t_Array u8 (sz 34))
+    Libcrux.Kem.Kyber.Matrix.sample_matrix_A v_K
+      (into_padded_array (sz 34) seed_for_A <: t_Array u8 (sz 34))
       true
   in
   let (prf_input: t_Array u8 (sz 33)):t_Array u8 (sz 33) =
-    Libcrux.Kem.Kyber.Conversions.into_padded_array (sz 33) seed_for_secret_and_error
+    into_padded_array (sz 33) seed_for_secret_and_error
   in
   let secret_as_ntt, domain_separator:(t_Array Libcrux.Kem.Kyber.Arithmetic.t_PolynomialRingElement
       v_K &
@@ -635,37 +583,16 @@ let generate_keypair
   let tt_as_ntt:t_Array Libcrux.Kem.Kyber.Arithmetic.t_PolynomialRingElement v_K =
     Libcrux.Kem.Kyber.Matrix.compute_As_plus_e v_K v_A_transpose secret_as_ntt error_as_ntt
   in
-  let public_key_serialized:Libcrux.Kem.Kyber.Conversions.t_UpdatableArray v_PUBLIC_KEY_SIZE =
-    Libcrux.Kem.Kyber.Conversions.impl__new v_PUBLIC_KEY_SIZE
-      (Rust_primitives.Hax.repeat 0uy v_PUBLIC_KEY_SIZE <: t_Array u8 v_PUBLIC_KEY_SIZE)
-  in
-  let public_key_serialized:Libcrux.Kem.Kyber.Conversions.t_UpdatableArray v_PUBLIC_KEY_SIZE =
-    Libcrux.Kem.Kyber.Conversions.f_push public_key_serialized
-      (Rust_primitives.unsize (serialize_key v_K v_RANKED_BYTES_PER_RING_ELEMENT tt_as_ntt
-            <:
-            t_Array u8 v_RANKED_BYTES_PER_RING_ELEMENT)
-        <:
-        t_Slice u8)
-  in
   let public_key_serialized:t_Array u8 v_PUBLIC_KEY_SIZE =
-    Libcrux.Kem.Kyber.Conversions.impl__array v_PUBLIC_KEY_SIZE
-      (Libcrux.Kem.Kyber.Conversions.f_push public_key_serialized seed_for_A
-        <:
-        Libcrux.Kem.Kyber.Conversions.t_UpdatableArray v_PUBLIC_KEY_SIZE)
+    serialize_public_key v_K v_RANKED_BYTES_PER_RING_ELEMENT v_PUBLIC_KEY_SIZE tt_as_ntt seed_for_A
   in
   let secret_key_serialized:t_Array u8 v_PRIVATE_KEY_SIZE =
-    serialize_key v_K v_PRIVATE_KEY_SIZE secret_as_ntt
+    serialize_secret_key v_K v_PRIVATE_KEY_SIZE secret_as_ntt
   in
-  let res = 
-  (Core.Convert.f_into secret_key_serialized, Core.Convert.f_into public_key_serialized
+  (secret_key_serialized, public_key_serialized
     <:
-    (Libcrux.Kem.Kyber.Types.t_PrivateKey v_PRIVATE_KEY_SIZE &
-      Libcrux.Kem.Kyber.Types.t_KyberPublicKey v_PUBLIC_KEY_SIZE)),
+    (t_Array u8 v_PRIVATE_KEY_SIZE & t_Array u8 v_PUBLIC_KEY_SIZE)),
   sampling_A_error
   <:
-  ((Libcrux.Kem.Kyber.Types.t_PrivateKey v_PRIVATE_KEY_SIZE &
-      Libcrux.Kem.Kyber.Types.t_KyberPublicKey v_PUBLIC_KEY_SIZE) &
-    Core.Option.t_Option Libcrux.Kem.Kyber.Types.t_Error) 
-  in
-  admit(); // Panic Freedom Proved, Functional Correctness Assumed.
-  res
+  ((t_Array u8 v_PRIVATE_KEY_SIZE & t_Array u8 v_PUBLIC_KEY_SIZE) &
+    Core.Option.t_Option Libcrux.Kem.Kyber.Types.t_Error)
