proofs/fstar/extraction-edited/Libcrux.Kem.Kyber.Serialize.fst
@@ -3,6 +3,150 @@ module Libcrux.Kem.Kyber.Serialize
 open Core
 open FStar.Mul
 
+let compress_coefficients_10_ (coefficient1 coefficient2 coefficient3 coefficient4: i32)
+    : (u8 & u8 & u8 & u8 & u8) =
+  let coef1:u8 = cast (coefficient1 &. 255l <: i32) <: u8 in
+  let coef2:u8 =
+    ((cast (coefficient2 &. 63l <: i32) <: u8) <<! 2l <: u8) |.
+    (cast ((coefficient1 >>! 8l <: i32) &. 3l <: i32) <: u8)
+  in
+  let coef3:u8 =
+    ((cast (coefficient3 &. 15l <: i32) <: u8) <<! 4l <: u8) |.
+    (cast ((coefficient2 >>! 6l <: i32) &. 15l <: i32) <: u8)
+  in
+  let coef4:u8 =
+    ((cast (coefficient4 &. 3l <: i32) <: u8) <<! 6l <: u8) |.
+    (cast ((coefficient3 >>! 4l <: i32) &. 63l <: i32) <: u8)
+  in
+  let coef5:u8 = cast ((coefficient4 >>! 2l <: i32) &. 255l <: i32) <: u8 in
+  coef1, coef2, coef3, coef4, coef5 <: (u8 & u8 & u8 & u8 & u8)
+
+let compress_coefficients_11_
+      (coefficient1 coefficient2 coefficient3 coefficient4 coefficient5 coefficient6 coefficient7 coefficient8:
+          i32)
+    : (u8 & u8 & u8 & u8 & u8 & u8 & u8 & u8 & u8 & u8 & u8) =
+  let coef1:u8 = cast (coefficient1 <: i32) <: u8 in
+  let coef2:u8 =
+    ((cast (coefficient2 &. 31l <: i32) <: u8) <<! 3l <: u8) |.
+    (cast (coefficient1 >>! 8l <: i32) <: u8)
+  in
+  let coef3:u8 =
+    ((cast (coefficient3 &. 3l <: i32) <: u8) <<! 6l <: u8) |.
+    (cast (coefficient2 >>! 5l <: i32) <: u8)
+  in
+  let coef4:u8 = cast ((coefficient3 >>! 2l <: i32) &. 255l <: i32) <: u8 in
+  let coef5:u8 =
+    ((cast (coefficient4 &. 127l <: i32) <: u8) <<! 1l <: u8) |.
+    (cast (coefficient3 >>! 10l <: i32) <: u8)
+  in
+  let coef6:u8 =
+    ((cast (coefficient5 &. 15l <: i32) <: u8) <<! 4l <: u8) |.
+    (cast (coefficient4 >>! 7l <: i32) <: u8)
+  in
+  let coef7:u8 =
+    ((cast (coefficient6 &. 1l <: i32) <: u8) <<! 7l <: u8) |.
+    (cast (coefficient5 >>! 4l <: i32) <: u8)
+  in
+  let coef8:u8 = cast ((coefficient6 >>! 1l <: i32) &. 255l <: i32) <: u8 in
+  let coef9:u8 =
+    ((cast (coefficient7 &. 63l <: i32) <: u8) <<! 2l <: u8) |.
+    (cast (coefficient6 >>! 9l <: i32) <: u8)
+  in
+  let coef10:u8 =
+    ((cast (coefficient8 &. 7l <: i32) <: u8) <<! 5l <: u8) |.
+    (cast (coefficient7 >>! 6l <: i32) <: u8)
+  in
+  let coef11:u8 = cast (coefficient8 >>! 3l <: i32) <: u8 in
+  coef1, coef2, coef3, coef4, coef5, coef6, coef7, coef8, coef9, coef10, coef11
+  <:
+  (u8 & u8 & u8 & u8 & u8 & u8 & u8 & u8 & u8 & u8 & u8)
+
+let compress_coefficients_3_ (coefficient1 coefficient2: u16) : (u8 & u8 & u8) =
+  let coef1:u8 = cast (coefficient1 &. 255us <: u16) <: u8 in
+  let coef2:u8 =
+    cast ((coefficient1 >>! 8l <: u16) |. ((coefficient2 &. 15us <: u16) <<! 4l <: u16) <: u16)
+    <:
+    u8
+  in
+  let coef3:u8 = cast ((coefficient2 >>! 4l <: u16) &. 255us <: u16) <: u8 in
+  coef1, coef2, coef3 <: (u8 & u8 & u8)
+
+let compress_coefficients_5_
+      (coefficient2 coefficient1 coefficient4 coefficient3 coefficient5 coefficient7 coefficient6 coefficient8:
+          u8)
+    : (u8 & u8 & u8 & u8 & u8) =
+  let coef1:u8 = ((coefficient2 &. 7uy <: u8) <<! 5l <: u8) |. coefficient1 in
+  let coef2:u8 =
+    (((coefficient4 &. 1uy <: u8) <<! 7l <: u8) |. (coefficient3 <<! 2l <: u8) <: u8) |.
+    (coefficient2 >>! 3l <: u8)
+  in
+  let coef3:u8 = ((coefficient5 &. 15uy <: u8) <<! 4l <: u8) |. (coefficient4 >>! 1l <: u8) in
+  let coef4:u8 =
+    (((coefficient7 &. 3uy <: u8) <<! 6l <: u8) |. (coefficient6 <<! 1l <: u8) <: u8) |.
+    (coefficient5 >>! 4l <: u8)
+  in
+  let coef5:u8 = (coefficient8 <<! 3l <: u8) |. (coefficient7 >>! 2l <: u8) in
+  coef1, coef2, coef3, coef4, coef5 <: (u8 & u8 & u8 & u8 & u8)
+
+let decompress_coefficients_10_ (byte2 byte1 byte3 byte4 byte5: i32) : (i32 & i32 & i32 & i32) =
+  let coefficient1:i32 = ((byte2 &. 3l <: i32) <<! 8l <: i32) |. (byte1 &. 255l <: i32) in
+  let coefficient2:i32 = ((byte3 &. 15l <: i32) <<! 6l <: i32) |. (byte2 >>! 2l <: i32) in
+  let coefficient3:i32 = ((byte4 &. 63l <: i32) <<! 4l <: i32) |. (byte3 >>! 4l <: i32) in
+  let coefficient4:i32 = (byte5 <<! 2l <: i32) |. (byte4 >>! 6l <: i32) in
+  coefficient1, coefficient2, coefficient3, coefficient4 <: (i32 & i32 & i32 & i32)
+
+let decompress_coefficients_11_
+      (byte2 byte1 byte3 byte5 byte4 byte6 byte7 byte9 byte8 byte10 byte11: i32)
+    : (i32 & i32 & i32 & i32 & i32 & i32 & i32 & i32) =
+  let coefficient1:i32 = ((byte2 &. 7l <: i32) <<! 8l <: i32) |. byte1 in
+  let coefficient2:i32 = ((byte3 &. 63l <: i32) <<! 5l <: i32) |. (byte2 >>! 3l <: i32) in
+  let coefficient3:i32 =
+    (((byte5 &. 1l <: i32) <<! 10l <: i32) |. (byte4 <<! 2l <: i32) <: i32) |. (byte3 >>! 6l <: i32)
+  in
+  let coefficient4:i32 = ((byte6 &. 15l <: i32) <<! 7l <: i32) |. (byte5 >>! 1l <: i32) in
+  let coefficient5:i32 = ((byte7 &. 127l <: i32) <<! 4l <: i32) |. (byte6 >>! 4l <: i32) in
+  let coefficient6:i32 =
+    (((byte9 &. 3l <: i32) <<! 9l <: i32) |. (byte8 <<! 1l <: i32) <: i32) |. (byte7 >>! 7l <: i32)
+  in
+  let coefficient7:i32 = ((byte10 &. 31l <: i32) <<! 6l <: i32) |. (byte9 >>! 2l <: i32) in
+  let coefficient8:i32 = (byte11 <<! 3l <: i32) |. (byte10 >>! 5l <: i32) in
+  coefficient1,
+  coefficient2,
+  coefficient3,
+  coefficient4,
+  coefficient5,
+  coefficient6,
+  coefficient7,
+  coefficient8
+  <:
+  (i32 & i32 & i32 & i32 & i32 & i32 & i32 & i32)
+
+let decompress_coefficients_4_ (byte: u8) : (i32 & i32) =
+  let coefficient1:i32 = cast (byte &. 15uy <: u8) <: i32 in
+  let coefficient2:i32 = cast ((byte >>! 4l <: u8) &. 15uy <: u8) <: i32 in
+  coefficient1, coefficient2 <: (i32 & i32)
+
+let decompress_coefficients_5_ (byte1 byte2 byte3 byte4 byte5: i32)
+    : (i32 & i32 & i32 & i32 & i32 & i32 & i32 & i32) =
+  let coefficient1:i32 = byte1 &. 31l in
+  let coefficient2:i32 = ((byte2 &. 3l <: i32) <<! 3l <: i32) |. (byte1 >>! 5l <: i32) in
+  let coefficient3:i32 = (byte2 >>! 2l <: i32) &. 31l in
+  let coefficient4:i32 = ((byte3 &. 15l <: i32) <<! 1l <: i32) |. (byte2 >>! 7l <: i32) in
+  let coefficient5:i32 = ((byte4 &. 1l <: i32) <<! 4l <: i32) |. (byte3 >>! 4l <: i32) in
+  let coefficient6:i32 = (byte4 >>! 1l <: i32) &. 31l in
+  let coefficient7:i32 = ((byte5 &. 7l <: i32) <<! 2l <: i32) |. (byte4 >>! 6l <: i32) in
+  let coefficient8:i32 = byte5 >>! 3l in
+  coefficient1,
+  coefficient2,
+  coefficient3,
+  coefficient4,
+  coefficient5,
+  coefficient6,
+  coefficient7,
+  coefficient8
+  <:
+  (i32 & i32 & i32 & i32 & i32 & i32 & i32 & i32)
+
 let compress_then_serialize_10_
       (v_OUT_LEN: usize)
       (re: Libcrux.Kem.Kyber.Arithmetic.t_PolynomialRingElement)
@@ -53,39 +197,33 @@ let compress_then_serialize_10_
                 <:
                 u16)
           in
+          let coef1, coef2, coef3, coef4, coef5:(u8 & u8 & u8 & u8 & u8) =
+            compress_coefficients_10_ coefficient1 coefficient2 coefficient3 coefficient4
+          in
           let serialized:t_Array u8 v_OUT_LEN =
             Rust_primitives.Hax.Monomorphized_update_at.update_at_usize serialized
               (sz 5 *! i <: usize)
-              (cast (coefficient1 &. 255l <: i32) <: u8)
+              coef1
           in
           let serialized:t_Array u8 v_OUT_LEN =
             Rust_primitives.Hax.Monomorphized_update_at.update_at_usize serialized
               ((sz 5 *! i <: usize) +! sz 1 <: usize)
-              (((cast (coefficient2 &. 63l <: i32) <: u8) <<! 2l <: u8) |.
-                (cast ((coefficient1 >>! 8l <: i32) &. 3l <: i32) <: u8)
-                <:
-                u8)
+              coef2
           in
           let serialized:t_Array u8 v_OUT_LEN =
             Rust_primitives.Hax.Monomorphized_update_at.update_at_usize serialized
               ((sz 5 *! i <: usize) +! sz 2 <: usize)
-              (((cast (coefficient3 &. 15l <: i32) <: u8) <<! 4l <: u8) |.
-                (cast ((coefficient2 >>! 6l <: i32) &. 15l <: i32) <: u8)
-                <:
-                u8)
+              coef3
           in
           let serialized:t_Array u8 v_OUT_LEN =
             Rust_primitives.Hax.Monomorphized_update_at.update_at_usize serialized
               ((sz 5 *! i <: usize) +! sz 3 <: usize)
-              (((cast (coefficient4 &. 3l <: i32) <: u8) <<! 6l <: u8) |.
-                (cast ((coefficient3 >>! 4l <: i32) &. 63l <: i32) <: u8)
-                <:
-                u8)
+              coef4
           in
           let serialized:t_Array u8 v_OUT_LEN =
             Rust_primitives.Hax.Monomorphized_update_at.update_at_usize serialized
               ((sz 5 *! i <: usize) +! sz 4 <: usize)
-              (cast ((coefficient4 >>! 2l <: i32) &. 255l <: i32) <: u8)
+              coef5
           in
           serialized)
   in
@@ -168,85 +306,83 @@ let compress_then_serialize_11_
                   )
                 <:
                 u16)
-          in 
+          in
+          let coef1, coef2, coef3, coef4, coef5, coef6, coef7, coef8, coef9, coef10, coef11:(u8 & u8 &
+            u8 &
+            u8 &
+            u8 &
+            u8 &
+            u8 &
+            u8 &
+            u8 &
+            u8 &
+            u8) =
+            compress_coefficients_11_ coefficient1
+              coefficient2
+              coefficient3
+              coefficient4
+              coefficient5
+              coefficient6
+              coefficient7
+              coefficient8
+          in
           let serialized:t_Array u8 v_OUT_LEN =
             Rust_primitives.Hax.Monomorphized_update_at.update_at_usize serialized
               (sz 11 *! i <: usize)
-              (cast (coefficient1 <: i32) <: u8)
+              coef1
           in
           let serialized:t_Array u8 v_OUT_LEN =
             Rust_primitives.Hax.Monomorphized_update_at.update_at_usize serialized
               ((sz 11 *! i <: usize) +! sz 1 <: usize)
-              (((cast (coefficient2 &. 31l <: i32) <: u8) <<! 3l <: u8) |.
-                (cast (coefficient1 >>! 8l <: i32) <: u8)
-                <:
-                u8)
+              coef2
           in
           let serialized:t_Array u8 v_OUT_LEN =
             Rust_primitives.Hax.Monomorphized_update_at.update_at_usize serialized
               ((sz 11 *! i <: usize) +! sz 2 <: usize)
-              (((cast (coefficient3 &. 3l <: i32) <: u8) <<! 6l <: u8) |.
-                (cast (coefficient2 >>! 5l <: i32) <: u8)
-                <:
-                u8)
+              coef3
           in
           let serialized:t_Array u8 v_OUT_LEN =
             Rust_primitives.Hax.Monomorphized_update_at.update_at_usize serialized
               ((sz 11 *! i <: usize) +! sz 3 <: usize)
-              (cast ((coefficient3 >>! 2l <: i32) &. 255l <: i32) <: u8)
+              coef4
           in
           let serialized:t_Array u8 v_OUT_LEN =
             Rust_primitives.Hax.Monomorphized_update_at.update_at_usize serialized
               ((sz 11 *! i <: usize) +! sz 4 <: usize)
-              (((cast (coefficient4 &. 127l <: i32) <: u8) <<! 1l <: u8) |.
-                (cast (coefficient3 >>! 10l <: i32) <: u8)
-                <:
-                u8)
-          in 
+              coef5
+          in
           let serialized:t_Array u8 v_OUT_LEN =
             Rust_primitives.Hax.Monomorphized_update_at.update_at_usize serialized
               ((sz 11 *! i <: usize) +! sz 5 <: usize)
-              (((cast (coefficient5 &. 15l <: i32) <: u8) <<! 4l <: u8) |.
-                (cast (coefficient4 >>! 7l <: i32) <: u8)
-                <:
-                u8)
+              coef6
           in
           let serialized:t_Array u8 v_OUT_LEN =
             Rust_primitives.Hax.Monomorphized_update_at.update_at_usize serialized
               ((sz 11 *! i <: usize) +! sz 6 <: usize)
-              (((cast (coefficient6 &. 1l <: i32) <: u8) <<! 7l <: u8) |.
-                (cast (coefficient5 >>! 4l <: i32) <: u8)
-                <:
-                u8)
-          in (* KB: F* blows up
+              coef7
+          in
           let serialized:t_Array u8 v_OUT_LEN =
             Rust_primitives.Hax.Monomorphized_update_at.update_at_usize serialized
               ((sz 11 *! i <: usize) +! sz 7 <: usize)
-              (cast ((coefficient6 >>! 1l <: i32) &. 255l <: i32) <: u8)
-          in 
+              coef8
+          in
           let serialized:t_Array u8 v_OUT_LEN =
             Rust_primitives.Hax.Monomorphized_update_at.update_at_usize serialized
               ((sz 11 *! i <: usize) +! sz 8 <: usize)
-              (((cast (coefficient7 &. 63l <: i32) <: u8) <<! 2l <: u8) |.
-                (cast (coefficient6 >>! 9l <: i32) <: u8)
-                <:
-                u8)
-          in 
+              coef9
+          in
           let serialized:t_Array u8 v_OUT_LEN =
             Rust_primitives.Hax.Monomorphized_update_at.update_at_usize serialized
               ((sz 11 *! i <: usize) +! sz 9 <: usize)
-              (((cast (coefficient8 &. 7l <: i32) <: u8) <<! 5l <: u8) |.
-                (cast (coefficient7 >>! 6l <: i32) <: u8)
-                <:
-                u8)
+              coef10
           in
           let serialized:t_Array u8 v_OUT_LEN =
             Rust_primitives.Hax.Monomorphized_update_at.update_at_usize serialized
               ((sz 11 *! i <: usize) +! sz 10 <: usize)
-              (cast (coefficient8 >>! 3l <: i32) <: u8)
-          in *)
-          serialized) 
-  in 
+              coef11
+          in
+          serialized)
+  in
   serialized
 
 let compress_then_serialize_4_
@@ -422,36 +558,40 @@ let compress_then_serialize_5_
             <:
             u8
           in
+          let coef1, coef2, coef3, coef4, coef5:(u8 & u8 & u8 & u8 & u8) =
+            compress_coefficients_5_ coefficient2
+              coefficient1
+              coefficient4
+              coefficient3
+              coefficient5
+              coefficient7
+              coefficient6
+              coefficient8
+          in
           let serialized:t_Array u8 v_OUT_LEN =
             Rust_primitives.Hax.Monomorphized_update_at.update_at_usize serialized
               (sz 5 *! i <: usize)
-              (((coefficient2 &. 7uy <: u8) <<! 5l <: u8) |. coefficient1 <: u8)
+              coef1
           in
           let serialized:t_Array u8 v_OUT_LEN =
             Rust_primitives.Hax.Monomorphized_update_at.update_at_usize serialized
               ((sz 5 *! i <: usize) +! sz 1 <: usize)
-              ((((coefficient4 &. 1uy <: u8) <<! 7l <: u8) |. (coefficient3 <<! 2l <: u8) <: u8) |.
-                (coefficient2 >>! 3l <: u8)
-                <:
-                u8)
+              coef2
           in
           let serialized:t_Array u8 v_OUT_LEN =
             Rust_primitives.Hax.Monomorphized_update_at.update_at_usize serialized
               ((sz 5 *! i <: usize) +! sz 2 <: usize)
-              (((coefficient5 &. 15uy <: u8) <<! 4l <: u8) |. (coefficient4 >>! 1l <: u8) <: u8)
+              coef3
           in
           let serialized:t_Array u8 v_OUT_LEN =
             Rust_primitives.Hax.Monomorphized_update_at.update_at_usize serialized
               ((sz 5 *! i <: usize) +! sz 3 <: usize)
-              ((((coefficient7 &. 3uy <: u8) <<! 6l <: u8) |. (coefficient6 <<! 1l <: u8) <: u8) |.
-                (coefficient5 >>! 4l <: u8)
-                <:
-                u8)
+              coef4
           in
           let serialized:t_Array u8 v_OUT_LEN =
             Rust_primitives.Hax.Monomorphized_update_at.update_at_usize serialized
               ((sz 5 *! i <: usize) +! sz 4 <: usize)
-              ((coefficient8 <<! 3l <: u8) |. (coefficient7 >>! 2l <: u8) <: u8)
+              coef5
           in
           serialized)
   in
@@ -501,24 +641,34 @@ let compress_then_serialize_message (re: Libcrux.Kem.Kyber.Arithmetic.t_Polynomi
   in
   serialized
 
-let compress_then_serialize_ring_element_u
+val compress_then_serialize_ring_element_u
       (v_COMPRESSION_FACTOR v_OUT_LEN: usize)
       (re: Libcrux.Kem.Kyber.Arithmetic.t_PolynomialRingElement)
-    : t_Array u8 v_OUT_LEN =
+    : Pure (t_Array u8 v_OUT_LEN)
+      (requires (v_COMPRESSION_FACTOR = sz 10 || v_COMPRESSION_FACTOR = sz 11)) 
+      (ensures (fun _ -> True)) 
+let compress_then_serialize_ring_element_u
+      (v_COMPRESSION_FACTOR v_OUT_LEN: usize)
+      (re: Libcrux.Kem.Kyber.Arithmetic.t_PolynomialRingElement) =
   let _:Prims.unit = () <: Prims.unit in
-  assume (v_COMPRESSION_FACTOR = sz 10 || v_COMPRESSION_FACTOR = sz 11);
-  mk_int_equiv_lemma #u32_inttype (v v_COMPRESSION_FACTOR);
+  Rust_primitives.Integers.mk_int_equiv_lemma #u32_inttype (v v_COMPRESSION_FACTOR);
   match cast (v_COMPRESSION_FACTOR <: usize) <: u32 with
   | 10ul -> compress_then_serialize_10_ v_OUT_LEN re
   | 11ul -> compress_then_serialize_11_ v_OUT_LEN re
+  | _ ->
+    Rust_primitives.Hax.never_to_any (Core.Panicking.panic "internal error: entered unreachable code"
+
+        <:
+        Rust_primitives.Hax.t_Never)
 
 let compress_then_serialize_ring_element_v
       (v_COMPRESSION_FACTOR v_OUT_LEN: usize)
       (re: Libcrux.Kem.Kyber.Arithmetic.t_PolynomialRingElement)
-    : t_Array u8 v_OUT_LEN =
+    : Pure (t_Array u8 v_OUT_LEN)
+      (requires (v_COMPRESSION_FACTOR = sz 4 || v_COMPRESSION_FACTOR = sz 5)) 
+      (ensures (fun _ -> True))  =
   let _:Prims.unit = () <: Prims.unit in
-  assume (v_COMPRESSION_FACTOR = sz 4 || v_COMPRESSION_FACTOR = sz 5);
-  mk_int_equiv_lemma #u32_inttype (v v_COMPRESSION_FACTOR);
+  Rust_primitives.Integers.mk_int_equiv_lemma #u32_inttype (v v_COMPRESSION_FACTOR);
   match cast (v_COMPRESSION_FACTOR <: usize) <: u32 with
   | 4ul -> compress_then_serialize_4_ v_OUT_LEN re
   | 5ul -> compress_then_serialize_5_ v_OUT_LEN re
@@ -528,7 +678,7 @@ let compress_then_serialize_ring_element_v
         <:
         Rust_primitives.Hax.t_Never)
 
-#push-options "--z3rlimit 1500"
+#push-options "--z3rlimit 500 --max_ifuel 2 --split_queries always"
 let deserialize_then_decompress_10_ (serialized: t_Slice u8)
     : Libcrux.Kem.Kyber.Arithmetic.t_PolynomialRingElement =
   let _:Prims.unit = () <: Prims.unit in
@@ -552,7 +702,9 @@ let deserialize_then_decompress_10_ (serialized: t_Slice u8)
           let byte3:i32 = cast (bytes.[ sz 2 ] <: u8) <: i32 in
           let byte4:i32 = cast (bytes.[ sz 3 ] <: u8) <: i32 in
           let byte5:i32 = cast (bytes.[ sz 4 ] <: u8) <: i32 in
-          let coefficient1:i32 = ((byte2 &. 3l <: i32) <<! 8l <: i32) |. (byte1 &. 255l <: i32) in
+          let coefficient1, coefficient2, coefficient3, coefficient4:(i32 & i32 & i32 & i32) =
+            decompress_coefficients_10_ byte2 byte1 byte3 byte4 byte5
+          in
           assume (v i * 4 + 4 <= 256);
           assume (Libcrux.Kem.Kyber.Compress.decompress_pre 10uy coefficient1);
           let re:Libcrux.Kem.Kyber.Arithmetic.t_PolynomialRingElement =
@@ -570,7 +722,6 @@ let deserialize_then_decompress_10_ (serialized: t_Slice u8)
             <:
             Libcrux.Kem.Kyber.Arithmetic.t_PolynomialRingElement
           in
-          let coefficient2:i32 = ((byte3 &. 15l <: i32) <<! 6l <: i32) |. (byte2 >>! 2l <: i32) in
           assume (Libcrux.Kem.Kyber.Compress.decompress_pre 10uy coefficient2);
           let re:Libcrux.Kem.Kyber.Arithmetic.t_PolynomialRingElement =
             {
@@ -587,7 +738,6 @@ let deserialize_then_decompress_10_ (serialized: t_Slice u8)
             <:
             Libcrux.Kem.Kyber.Arithmetic.t_PolynomialRingElement
           in
-          let coefficient3:i32 = ((byte4 &. 63l <: i32) <<! 4l <: i32) |. (byte3 >>! 4l <: i32) in
           assume (Libcrux.Kem.Kyber.Compress.decompress_pre 10uy coefficient3);
           let re:Libcrux.Kem.Kyber.Arithmetic.t_PolynomialRingElement =
             {
@@ -604,7 +754,6 @@ let deserialize_then_decompress_10_ (serialized: t_Slice u8)
             <:
             Libcrux.Kem.Kyber.Arithmetic.t_PolynomialRingElement
           in
-          let coefficient4:i32 = (byte5 <<! 2l <: i32) |. (byte4 >>! 6l <: i32) in
           assume (Libcrux.Kem.Kyber.Compress.decompress_pre 10uy coefficient4);
           let re:Libcrux.Kem.Kyber.Arithmetic.t_PolynomialRingElement =
             {
@@ -624,9 +773,7 @@ let deserialize_then_decompress_10_ (serialized: t_Slice u8)
           re)
   in
   re
-#pop-options
 
-#push-options "--z3rlimit 500 --max_ifuel 2 --split_queries always"
 let deserialize_then_decompress_11_ (serialized: t_Slice u8)
     : Libcrux.Kem.Kyber.Arithmetic.t_PolynomialRingElement =
   let _:Prims.unit = () <: Prims.unit in
@@ -657,8 +804,18 @@ let deserialize_then_decompress_11_ (serialized: t_Slice u8)
           let byte9:i32 = cast (bytes.[ sz 8 ] <: u8) <: i32 in
           let byte10:i32 = cast (bytes.[ sz 9 ] <: u8) <: i32 in
           let byte11:i32 = cast (bytes.[ sz 10 ] <: u8) <: i32 in
-          let coefficient1:i32 = ((byte2 &. 7l <: i32) <<! 8l <: i32) |. byte1 in
-          admit();
+          let
+          coefficient1,
+          coefficient2,
+          coefficient3,
+          coefficient4,
+          coefficient5,
+          coefficient6,
+          coefficient7,
+          coefficient8:(i32 & i32 & i32 & i32 & i32 & i32 & i32 & i32) =
+            decompress_coefficients_11_ byte2 byte1 byte3 byte5 byte4 byte6 byte7 byte9 byte8 byte10
+              byte11
+          in
           assume (Libcrux.Kem.Kyber.Compress.decompress_pre 11uy coefficient1);
           let re:Libcrux.Kem.Kyber.Arithmetic.t_PolynomialRingElement =
             {
@@ -675,7 +832,6 @@ let deserialize_then_decompress_11_ (serialized: t_Slice u8)
             <:
             Libcrux.Kem.Kyber.Arithmetic.t_PolynomialRingElement
           in
-          let coefficient2:i32 = ((byte3 &. 63l <: i32) <<! 5l <: i32) |. (byte2 >>! 3l <: i32) in
           assume (Libcrux.Kem.Kyber.Compress.decompress_pre 11uy coefficient2);
           let re:Libcrux.Kem.Kyber.Arithmetic.t_PolynomialRingElement =
             {
@@ -691,10 +847,6 @@ let deserialize_then_decompress_11_ (serialized: t_Slice u8)
             }
             <:
             Libcrux.Kem.Kyber.Arithmetic.t_PolynomialRingElement
-          in
-          let coefficient3:i32 =
-            (((byte5 &. 1l <: i32) <<! 10l <: i32) |. (byte4 <<! 2l <: i32) <: i32) |.
-            (byte3 >>! 6l <: i32)
           in
           assume (Libcrux.Kem.Kyber.Compress.decompress_pre 11uy coefficient3);
           let re:Libcrux.Kem.Kyber.Arithmetic.t_PolynomialRingElement =
@@ -712,7 +864,6 @@ let deserialize_then_decompress_11_ (serialized: t_Slice u8)
             <:
             Libcrux.Kem.Kyber.Arithmetic.t_PolynomialRingElement
           in
-          let coefficient4:i32 = ((byte6 &. 15l <: i32) <<! 7l <: i32) |. (byte5 >>! 1l <: i32) in
           assume (Libcrux.Kem.Kyber.Compress.decompress_pre 11uy coefficient4);
           let re:Libcrux.Kem.Kyber.Arithmetic.t_PolynomialRingElement =
             {
@@ -729,7 +880,6 @@ let deserialize_then_decompress_11_ (serialized: t_Slice u8)
             <:
             Libcrux.Kem.Kyber.Arithmetic.t_PolynomialRingElement
           in
-          let coefficient5:i32 = ((byte7 &. 127l <: i32) <<! 4l <: i32) |. (byte6 >>! 4l <: i32) in
           assume (Libcrux.Kem.Kyber.Compress.decompress_pre 11uy coefficient5);
           let re:Libcrux.Kem.Kyber.Arithmetic.t_PolynomialRingElement =
             {
@@ -746,12 +896,8 @@ let deserialize_then_decompress_11_ (serialized: t_Slice u8)
             <:
             Libcrux.Kem.Kyber.Arithmetic.t_PolynomialRingElement
           in
-          let coefficient6:i32 =
-            (((byte9 &. 3l <: i32) <<! 9l <: i32) |. (byte8 <<! 1l <: i32) <: i32) |.
-            (byte7 >>! 7l <: i32)
-          in
           assume (Libcrux.Kem.Kyber.Compress.decompress_pre 11uy coefficient6);
-         let re:Libcrux.Kem.Kyber.Arithmetic.t_PolynomialRingElement =
+          let re:Libcrux.Kem.Kyber.Arithmetic.t_PolynomialRingElement =
             {
               re with
               Libcrux.Kem.Kyber.Arithmetic.f_coefficients
@@ -766,7 +912,6 @@ let deserialize_then_decompress_11_ (serialized: t_Slice u8)
             <:
             Libcrux.Kem.Kyber.Arithmetic.t_PolynomialRingElement
           in
-          let coefficient7:i32 = ((byte10 &. 31l <: i32) <<! 6l <: i32) |. (byte9 >>! 2l <: i32) in
           assume (Libcrux.Kem.Kyber.Compress.decompress_pre 11uy coefficient7);
           let re:Libcrux.Kem.Kyber.Arithmetic.t_PolynomialRingElement =
             {
@@ -783,7 +928,6 @@ let deserialize_then_decompress_11_ (serialized: t_Slice u8)
             <:
             Libcrux.Kem.Kyber.Arithmetic.t_PolynomialRingElement
           in
-          let coefficient8:i32 = (byte11 <<! 3l <: i32) |. (byte10 >>! 5l <: i32) in
           assume (Libcrux.Kem.Kyber.Compress.decompress_pre 11uy coefficient8);
           let re:Libcrux.Kem.Kyber.Arithmetic.t_PolynomialRingElement =
             {
@@ -803,7 +947,6 @@ let deserialize_then_decompress_11_ (serialized: t_Slice u8)
           re)
   in
   re
-#pop-options
 
 let deserialize_then_decompress_4_ (serialized: t_Slice u8)
     : Libcrux.Kem.Kyber.Arithmetic.t_PolynomialRingElement =
@@ -823,7 +966,7 @@ let deserialize_then_decompress_4_ (serialized: t_Slice u8)
           let re:Libcrux.Kem.Kyber.Arithmetic.t_PolynomialRingElement = re in
           let i, byte:(usize & u8) = temp_1_ in
           assume (v i * 2 + 2 <= 256);
-          let coefficient1:i32 = cast (byte &. 15uy <: u8) <: i32 in
+          let coefficient1, coefficient2:(i32 & i32) = decompress_coefficients_4_ byte in
           assume (Libcrux.Kem.Kyber.Compress.decompress_pre 4uy coefficient1);
           let re:Libcrux.Kem.Kyber.Arithmetic.t_PolynomialRingElement =
             {
@@ -840,7 +983,6 @@ let deserialize_then_decompress_4_ (serialized: t_Slice u8)
             <:
             Libcrux.Kem.Kyber.Arithmetic.t_PolynomialRingElement
           in
-          let coefficient2:i32 = cast ((byte >>! 4l <: u8) &. 15uy <: u8) <: i32 in
           assume (Libcrux.Kem.Kyber.Compress.decompress_pre 4uy coefficient2);
           let re:Libcrux.Kem.Kyber.Arithmetic.t_PolynomialRingElement =
             {
@@ -885,7 +1027,17 @@ let deserialize_then_decompress_5_ (serialized: t_Slice u8)
           let byte3:i32 = cast (bytes.[ sz 2 ] <: u8) <: i32 in
           let byte4:i32 = cast (bytes.[ sz 3 ] <: u8) <: i32 in
           let byte5:i32 = cast (bytes.[ sz 4 ] <: u8) <: i32 in
-          let coefficient1:i32 = byte1 &. 31l in
+          let
+          coefficient1,
+          coefficient2,
+          coefficient3,
+          coefficient4,
+          coefficient5,
+          coefficient6,
+          coefficient7,
+          coefficient8:(i32 & i32 & i32 & i32 & i32 & i32 & i32 & i32) =
+            decompress_coefficients_5_ byte1 byte2 byte3 byte4 byte5
+          in
           assume (Libcrux.Kem.Kyber.Compress.decompress_pre 5uy coefficient1);
           let re:Libcrux.Kem.Kyber.Arithmetic.t_PolynomialRingElement =
             {
@@ -902,8 +1054,6 @@ let deserialize_then_decompress_5_ (serialized: t_Slice u8)
             <:
             Libcrux.Kem.Kyber.Arithmetic.t_PolynomialRingElement
           in
-          admit();
-          let coefficient2:i32 = ((byte2 &. 3l <: i32) <<! 3l <: i32) |. (byte1 >>! 5l <: i32) in
           assume (Libcrux.Kem.Kyber.Compress.decompress_pre 5uy coefficient2);
           let re:Libcrux.Kem.Kyber.Arithmetic.t_PolynomialRingElement =
             {
@@ -920,7 +1070,6 @@ let deserialize_then_decompress_5_ (serialized: t_Slice u8)
             <:
             Libcrux.Kem.Kyber.Arithmetic.t_PolynomialRingElement
           in
-          let coefficient3:i32 = (byte2 >>! 2l <: i32) &. 31l in
           assume (Libcrux.Kem.Kyber.Compress.decompress_pre 5uy coefficient3);
           let re:Libcrux.Kem.Kyber.Arithmetic.t_PolynomialRingElement =
             {
@@ -937,7 +1086,6 @@ let deserialize_then_decompress_5_ (serialized: t_Slice u8)
             <:
             Libcrux.Kem.Kyber.Arithmetic.t_PolynomialRingElement
           in
-          let coefficient4:i32 = ((byte3 &. 15l <: i32) <<! 1l <: i32) |. (byte2 >>! 7l <: i32) in
           assume (Libcrux.Kem.Kyber.Compress.decompress_pre 5uy coefficient4);
           let re:Libcrux.Kem.Kyber.Arithmetic.t_PolynomialRingElement =
             {
@@ -954,7 +1102,7 @@ let deserialize_then_decompress_5_ (serialized: t_Slice u8)
             <:
             Libcrux.Kem.Kyber.Arithmetic.t_PolynomialRingElement
           in
-          let coefficient5:i32 = ((byte4 &. 1l <: i32) <<! 4l <: i32) |. (byte3 >>! 4l <: i32) in
+          admit();
           assume (Libcrux.Kem.Kyber.Compress.decompress_pre 5uy coefficient5);
           let re:Libcrux.Kem.Kyber.Arithmetic.t_PolynomialRingElement =
             {
@@ -971,7 +1119,6 @@ let deserialize_then_decompress_5_ (serialized: t_Slice u8)
             <:
             Libcrux.Kem.Kyber.Arithmetic.t_PolynomialRingElement
           in
-          let coefficient6:i32 = (byte4 >>! 1l <: i32) &. 31l in
           assume (Libcrux.Kem.Kyber.Compress.decompress_pre 5uy coefficient6);
           let re:Libcrux.Kem.Kyber.Arithmetic.t_PolynomialRingElement =
             {
@@ -988,7 +1135,6 @@ let deserialize_then_decompress_5_ (serialized: t_Slice u8)
             <:
             Libcrux.Kem.Kyber.Arithmetic.t_PolynomialRingElement
           in
-          let coefficient7:i32 = ((byte5 &. 7l <: i32) <<! 2l <: i32) |. (byte4 >>! 6l <: i32) in
           assume (Libcrux.Kem.Kyber.Compress.decompress_pre 5uy coefficient7);
           let re:Libcrux.Kem.Kyber.Arithmetic.t_PolynomialRingElement =
             {
@@ -1005,7 +1151,6 @@ let deserialize_then_decompress_5_ (serialized: t_Slice u8)
             <:
             Libcrux.Kem.Kyber.Arithmetic.t_PolynomialRingElement
           in
-          let coefficient8:i32 = byte5 >>! 3l in
           assume (Libcrux.Kem.Kyber.Compress.decompress_pre 5uy coefficient8);
           let re:Libcrux.Kem.Kyber.Arithmetic.t_PolynomialRingElement =
             {
@@ -1025,6 +1170,7 @@ let deserialize_then_decompress_5_ (serialized: t_Slice u8)
           re)
   in
   re
+#pop-options
 
 let deserialize_then_decompress_message (serialized: t_Array u8 (sz 32))
     : Libcrux.Kem.Kyber.Arithmetic.t_PolynomialRingElement =
@@ -1191,24 +1337,23 @@ let serialize_uncompressed_ring_element (re: Libcrux.Kem.Kyber.Arithmetic.t_Poly
           let coefficient2:u16 =
             Libcrux.Kem.Kyber.Arithmetic.to_unsigned_representative (coefficients.[ sz 1 ] <: i32)
           in
+          let coef1, coef2, coef3:(u8 & u8 & u8) =
+            compress_coefficients_3_ coefficient1 coefficient2
+          in
           let serialized:t_Array u8 (sz 384) =
             Rust_primitives.Hax.Monomorphized_update_at.update_at_usize serialized
               (sz 3 *! i <: usize)
-              (cast (coefficient1 &. 255us <: u16) <: u8)
+              coef1
           in
           let serialized:t_Array u8 (sz 384) =
             Rust_primitives.Hax.Monomorphized_update_at.update_at_usize serialized
               ((sz 3 *! i <: usize) +! sz 1 <: usize)
-              (cast ((coefficient1 >>! 8l <: u16) |. ((coefficient2 &. 15us <: u16) <<! 4l <: u16)
-                    <:
-                    u16)
-                <:
-                u8)
+              coef2
           in
           let serialized:t_Array u8 (sz 384) =
             Rust_primitives.Hax.Monomorphized_update_at.update_at_usize serialized
               ((sz 3 *! i <: usize) +! sz 2 <: usize)
-              (cast ((coefficient2 >>! 4l <: u16) &. 255us <: u16) <: u8)
+              coef3
           in
           serialized)
   in
