proofs/fstar/extraction-edited/Libcrux.Kem.Kyber.fst
@@ -10,12 +10,118 @@ let v_KEY_GENERATION_SEED_SIZE: usize =
   Libcrux.Kem.Kyber.Constants.v_CPA_PKE_KEY_GENERATION_SEED_SIZE +!
   Libcrux.Kem.Kyber.Constants.v_SHARED_SECRET_SIZE
 
+let serialize_kem_secret_key
+      (v_SERIALIZED_KEY_LEN: usize)
+      (private_key public_key implicit_rejection_value: t_Slice u8) =
+  let out:t_Array u8 v_SERIALIZED_KEY_LEN = Rust_primitives.Hax.repeat 0uy v_SERIALIZED_KEY_LEN in
+  let pointer:usize = sz 0 in
+  let out:t_Array u8 v_SERIALIZED_KEY_LEN =
+    Rust_primitives.Hax.Monomorphized_update_at.update_at_range out
+      ({
+          Core.Ops.Range.f_start = pointer;
+          Core.Ops.Range.f_end = pointer +! (Core.Slice.impl__len private_key <: usize) <: usize
+        }
+        <:
+        Core.Ops.Range.t_Range usize)
+      (Core.Slice.impl__copy_from_slice (out.[ {
+                Core.Ops.Range.f_start = pointer;
+                Core.Ops.Range.f_end
+                =
+                pointer +! (Core.Slice.impl__len private_key <: usize) <: usize
+              }
+              <:
+              Core.Ops.Range.t_Range usize ]
+            <:
+            t_Slice u8)
+          private_key
+        <:
+        t_Slice u8)
+  in
+  let pointer:usize = pointer +! (Core.Slice.impl__len private_key <: usize) in
+  let out:t_Array u8 v_SERIALIZED_KEY_LEN =
+    Rust_primitives.Hax.Monomorphized_update_at.update_at_range out
+      ({
+          Core.Ops.Range.f_start = pointer;
+          Core.Ops.Range.f_end = pointer +! (Core.Slice.impl__len public_key <: usize) <: usize
+        }
+        <:
+        Core.Ops.Range.t_Range usize)
+      (Core.Slice.impl__copy_from_slice (out.[ {
+                Core.Ops.Range.f_start = pointer;
+                Core.Ops.Range.f_end
+                =
+                pointer +! (Core.Slice.impl__len public_key <: usize) <: usize
+              }
+              <:
+              Core.Ops.Range.t_Range usize ]
+            <:
+            t_Slice u8)
+          public_key
+        <:
+        t_Slice u8)
+  in
+  let pointer:usize = pointer +! (Core.Slice.impl__len public_key <: usize) in
+  let out:t_Array u8 v_SERIALIZED_KEY_LEN =
+    Rust_primitives.Hax.Monomorphized_update_at.update_at_range out
+      ({
+          Core.Ops.Range.f_start = pointer;
+          Core.Ops.Range.f_end = pointer +! Libcrux.Kem.Kyber.Constants.v_H_DIGEST_SIZE <: usize
+        }
+        <:
+        Core.Ops.Range.t_Range usize)
+      (Core.Slice.impl__copy_from_slice (out.[ {
+                Core.Ops.Range.f_start = pointer;
+                Core.Ops.Range.f_end
+                =
+                pointer +! Libcrux.Kem.Kyber.Constants.v_H_DIGEST_SIZE <: usize
+              }
+              <:
+              Core.Ops.Range.t_Range usize ]
+            <:
+            t_Slice u8)
+          (Rust_primitives.unsize (Libcrux.Kem.Kyber.Hash_functions.v_H public_key
+                <:
+                t_Array u8 (sz 32))
+            <:
+            t_Slice u8)
+        <:
+        t_Slice u8)
+  in
+  let pointer:usize = pointer +! Libcrux.Kem.Kyber.Constants.v_H_DIGEST_SIZE in
+  let out:t_Array u8 v_SERIALIZED_KEY_LEN =
+    Rust_primitives.Hax.Monomorphized_update_at.update_at_range out
+      ({
+          Core.Ops.Range.f_start = pointer;
+          Core.Ops.Range.f_end
+          =
+          pointer +! (Core.Slice.impl__len implicit_rejection_value <: usize) <: usize
+        }
+        <:
+        Core.Ops.Range.t_Range usize)
+      (Core.Slice.impl__copy_from_slice (out.[ {
+                Core.Ops.Range.f_start = pointer;
+                Core.Ops.Range.f_end
+                =
+                pointer +! (Core.Slice.impl__len implicit_rejection_value <: usize) <: usize
+              }
+              <:
+              Core.Ops.Range.t_Range usize ]
+            <:
+            t_Slice u8)
+          implicit_rejection_value
+        <:
+        t_Slice u8)
+  in
+  admit(); // P-F
+  out
+
 let decapsulate #p
-      v_K v_SECRET_KEY_SIZE v_CPA_SECRET_KEY_SIZE v_PUBLIC_KEY_SIZE v_CIPHERTEXT_SIZE v_T_AS_NTT_ENCODED_SIZE v_C1_SIZE v_C2_SIZE v_VECTOR_U_COMPRESSION_FACTOR v_VECTOR_V_COMPRESSION_FACTOR v_C1_BLOCK_SIZE v_ETA1 v_ETA1_RANDOMNESS_SIZE v_ETA2 v_ETA2_RANDOMNESS_SIZE v_IMPLICIT_REJECTION_HASH_INPUT_SIZE
+      (v_K v_SECRET_KEY_SIZE v_CPA_SECRET_KEY_SIZE v_PUBLIC_KEY_SIZE v_CIPHERTEXT_SIZE v_T_AS_NTT_ENCODED_SIZE v_C1_SIZE v_C2_SIZE v_VECTOR_U_COMPRESSION_FACTOR v_VECTOR_V_COMPRESSION_FACTOR v_C1_BLOCK_SIZE v_ETA1 v_ETA1_RANDOMNESS_SIZE v_ETA2 v_ETA2_RANDOMNESS_SIZE v_IMPLICIT_REJECTION_HASH_INPUT_SIZE:
+          usize)
       (secret_key: Libcrux.Kem.Kyber.Types.t_KyberPrivateKey v_SECRET_KEY_SIZE)
-      (ciphertext: Libcrux.Kem.Kyber.Types.t_KyberCiphertext v_CIPHERTEXT_SIZE) = 
+      (ciphertext: Libcrux.Kem.Kyber.Types.t_KyberCiphertext v_CIPHERTEXT_SIZE) =
   let ind_cpa_secret_key, secret_key:(t_Slice u8 & t_Slice u8) =
-    Libcrux.Kem.Kyber.Types.impl_18__split_at v_SECRET_KEY_SIZE secret_key v_CPA_SECRET_KEY_SIZE
+    Libcrux.Kem.Kyber.Types.impl_12__split_at v_SECRET_KEY_SIZE secret_key v_CPA_SECRET_KEY_SIZE
   in
   let ind_cpa_public_key, secret_key:(t_Slice u8 & t_Slice u8) =
     Core.Slice.impl__split_at secret_key v_PUBLIC_KEY_SIZE
@@ -23,9 +129,6 @@ let decapsulate #p
   let ind_cpa_public_key_hash, implicit_rejection_value:(t_Slice u8 & t_Slice u8) =
     Core.Slice.impl__split_at secret_key Libcrux.Kem.Kyber.Constants.v_H_DIGEST_SIZE
   in
-  assert (length implicit_rejection_value = v_SECRET_KEY_SIZE -! v_CPA_SECRET_KEY_SIZE -! v_PUBLIC_KEY_SIZE -! Libcrux.Kem.Kyber.Constants.v_H_DIGEST_SIZE);
-  assert (length implicit_rejection_value = Spec.Kyber.v_SHARED_SECRET_SIZE);
-  assert (Spec.Kyber.v_SHARED_SECRET_SIZE <=. Spec.Kyber.v_IMPLICIT_REJECTION_HASH_INPUT_SIZE p);
   let decrypted:t_Array u8 (sz 32) =
     Libcrux.Kem.Kyber.Ind_cpa.decrypt #p v_K
       v_CIPHERTEXT_SIZE
@@ -33,10 +136,10 @@ let decapsulate #p
       v_VECTOR_U_COMPRESSION_FACTOR
       v_VECTOR_V_COMPRESSION_FACTOR
       ind_cpa_secret_key
-      ciphertext
+      ciphertext.Libcrux.Kem.Kyber.Types.f_value
   in
   let (to_hash: t_Array u8 (sz 64)):t_Array u8 (sz 64) =
-    Libcrux.Kem.Kyber.Conversions.into_padded_array (sz 64)
+    Libcrux.Kem.Kyber.Ind_cpa.into_padded_array (sz 64)
       (Rust_primitives.unsize decrypted <: t_Slice u8)
   in
   let to_hash:t_Array u8 (sz 64) =
@@ -63,9 +166,12 @@ let decapsulate #p
     Core.Slice.impl__split_at (Rust_primitives.unsize hashed <: t_Slice u8)
       Libcrux.Kem.Kyber.Constants.v_SHARED_SECRET_SIZE
   in
+  assert (length implicit_rejection_value = v_SECRET_KEY_SIZE -! v_CPA_SECRET_KEY_SIZE -! v_PUBLIC_KEY_SIZE -! Libcrux.Kem.Kyber.Constants.v_H_DIGEST_SIZE);
+  assert (length implicit_rejection_value = Spec.Kyber.v_SHARED_SECRET_SIZE);
+  assert (Spec.Kyber.v_SHARED_SECRET_SIZE <=. Spec.Kyber.v_IMPLICIT_REJECTION_HASH_INPUT_SIZE p);
   let (to_hash: t_Array u8 v_IMPLICIT_REJECTION_HASH_INPUT_SIZE):t_Array u8
     v_IMPLICIT_REJECTION_HASH_INPUT_SIZE =
-    Libcrux.Kem.Kyber.Conversions.into_padded_array v_IMPLICIT_REJECTION_HASH_INPUT_SIZE
+    Libcrux.Kem.Kyber.Ind_cpa.into_padded_array v_IMPLICIT_REJECTION_HASH_INPUT_SIZE
       implicit_rejection_value
   in
   let to_hash:t_Array u8 v_IMPLICIT_REJECTION_HASH_INPUT_SIZE =
@@ -87,7 +193,7 @@ let decapsulate #p
   let (implicit_rejection_shared_secret: t_Array u8 (sz 32)):t_Array u8 (sz 32) =
     Libcrux.Kem.Kyber.Hash_functions.v_PRF (sz 32) (Rust_primitives.unsize to_hash <: t_Slice u8)
   in
-  let expected_ciphertext, _:(Libcrux.Kem.Kyber.Types.t_KyberCiphertext v_CIPHERTEXT_SIZE &
+  let expected_ciphertext, _:(t_Array u8 v_CIPHERTEXT_SIZE &
     Core.Option.t_Option Libcrux.Kem.Kyber.Types.t_Error) =
     Libcrux.Kem.Kyber.Ind_cpa.encrypt #p v_K v_CIPHERTEXT_SIZE v_T_AS_NTT_ENCODED_SIZE v_C1_SIZE
       v_C2_SIZE v_VECTOR_U_COMPRESSION_FACTOR v_VECTOR_V_COMPRESSION_FACTOR v_C1_BLOCK_SIZE v_ETA1
@@ -97,12 +203,13 @@ let decapsulate #p
   let selector:u8 =
     Libcrux.Kem.Kyber.Constant_time_ops.compare_ciphertexts_in_constant_time v_CIPHERTEXT_SIZE
       (Core.Convert.f_as_ref ciphertext <: t_Slice u8)
-      (Core.Convert.f_as_ref expected_ciphertext <: t_Slice u8)
+      (Rust_primitives.unsize expected_ciphertext <: t_Slice u8)
   in
   let res = 
   Libcrux.Kem.Kyber.Constant_time_ops.select_shared_secret_in_constant_time shared_secret
     (Rust_primitives.unsize implicit_rejection_shared_secret <: t_Slice u8)
-    selector in
+    selector
+  in
   res
 
 let encapsulate #p
@@ -111,7 +218,7 @@ let encapsulate #p
       (public_key: Libcrux.Kem.Kyber.Types.t_KyberPublicKey v_PUBLIC_KEY_SIZE)
       (randomness: t_Array u8 (sz 32)) =
   let (to_hash: t_Array u8 (sz 64)):t_Array u8 (sz 64) =
-    Libcrux.Kem.Kyber.Conversions.into_padded_array (sz 64)
+    Libcrux.Kem.Kyber.Ind_cpa.into_padded_array (sz 64)
       (Rust_primitives.unsize randomness <: t_Slice u8)
   in
   let to_hash:t_Array u8 (sz 64) =
@@ -126,7 +233,7 @@ let encapsulate #p
               Core.Ops.Range.t_RangeFrom usize ]
             <:
             t_Slice u8)
-          (Rust_primitives.unsize (Libcrux.Kem.Kyber.Hash_functions.v_H (Rust_primitives.unsize (Libcrux.Kem.Kyber.Types.impl_24__as_slice
+          (Rust_primitives.unsize (Libcrux.Kem.Kyber.Hash_functions.v_H (Rust_primitives.unsize (Libcrux.Kem.Kyber.Types.impl_18__as_slice
                           v_PUBLIC_KEY_SIZE
                           public_key
                         <:
@@ -143,6 +250,7 @@ let encapsulate #p
   assert (Seq.slice to_hash 0 (v Libcrux.Kem.Kyber.Constants.v_H_DIGEST_SIZE) == randomness);
   Spec.Kyber.lemma_slice_append to_hash randomness (Spec.Kyber.v_H public_key.f_value) Libcrux.Kem.Kyber.Constants.v_H_DIGEST_SIZE;
   assert (to_hash == Spec.Kyber.concat randomness (Spec.Kyber.v_H public_key.f_value));
+
   let hashed:t_Array u8 (sz 64) =
     Libcrux.Kem.Kyber.Hash_functions.v_G (Rust_primitives.unsize to_hash <: t_Slice u8)
   in
@@ -150,12 +258,12 @@ let encapsulate #p
     Core.Slice.impl__split_at (Rust_primitives.unsize hashed <: t_Slice u8)
       Libcrux.Kem.Kyber.Constants.v_SHARED_SECRET_SIZE
   in
-  let ciphertext, sampling_a_error:(Libcrux.Kem.Kyber.Types.t_KyberCiphertext v_CIPHERTEXT_SIZE &
+  let ciphertext, sampling_a_error:(t_Array u8 v_CIPHERTEXT_SIZE &
     Core.Option.t_Option Libcrux.Kem.Kyber.Types.t_Error) =
     Libcrux.Kem.Kyber.Ind_cpa.encrypt #p v_K v_CIPHERTEXT_SIZE v_T_AS_NTT_ENCODED_SIZE v_C1_SIZE
       v_C2_SIZE v_VECTOR_U_COMPRESSION_FACTOR v_VECTOR_V_COMPRESSION_FACTOR v_VECTOR_U_BLOCK_LEN
       v_ETA1 v_ETA1_RANDOMNESS_SIZE v_ETA2 v_ETA2_RANDOMNESS_SIZE
-      (Rust_primitives.unsize (Libcrux.Kem.Kyber.Types.impl_24__as_slice v_PUBLIC_KEY_SIZE
+      (Rust_primitives.unsize (Libcrux.Kem.Kyber.Types.impl_18__as_slice v_PUBLIC_KEY_SIZE
               public_key
             <:
             t_Array u8 v_PUBLIC_KEY_SIZE)
@@ -172,7 +280,7 @@ let encapsulate #p
       Libcrux.Kem.Kyber.Types.t_Error
   | Core.Option.Option_None  ->
     Core.Result.Result_Ok
-    (ciphertext,
+    (Core.Convert.f_into ciphertext,
       Core.Result.impl__unwrap (Core.Convert.f_try_into shared_secret
           <:
           Core.Result.t_Result (t_Array u8 (sz 32)) Core.Array.t_TryFromSliceError)
@@ -183,12 +291,12 @@ let encapsulate #p
       (Libcrux.Kem.Kyber.Types.t_KyberCiphertext v_CIPHERTEXT_SIZE & t_Array u8 (sz 32))
       Libcrux.Kem.Kyber.Types.t_Error
   in
-  res 
+  res
 
 let generate_keypair #p
       (v_K v_CPA_PRIVATE_KEY_SIZE v_PRIVATE_KEY_SIZE v_PUBLIC_KEY_SIZE v_BYTES_PER_RING_ELEMENT v_ETA1 v_ETA1_RANDOMNESS_SIZE:
           usize)
-      (randomness: t_Array u8 (sz 64)) = 
+      (randomness: t_Array u8 (sz 64)) =
   let ind_cpa_keypair_randomness:t_Slice u8 =
     randomness.[ {
         Core.Ops.Range.f_start = sz 0;
@@ -204,9 +312,8 @@ let generate_keypair #p
       <:
       Core.Ops.Range.t_RangeFrom usize ]
   in
-  let (ind_cpa_private_key, public_key), sampling_a_error:((Libcrux.Kem.Kyber.Types.t_PrivateKey
-      v_CPA_PRIVATE_KEY_SIZE &
-      Libcrux.Kem.Kyber.Types.t_KyberPublicKey v_PUBLIC_KEY_SIZE) &
+  let (ind_cpa_private_key, public_key), sampling_a_error:((t_Array u8 v_CPA_PRIVATE_KEY_SIZE &
+      t_Array u8 v_PUBLIC_KEY_SIZE) &
     Core.Option.t_Option Libcrux.Kem.Kyber.Types.t_Error) =
     Libcrux.Kem.Kyber.Ind_cpa.generate_keypair #p v_K
       v_CPA_PRIVATE_KEY_SIZE
@@ -217,39 +324,34 @@ let generate_keypair #p
       ind_cpa_keypair_randomness
   in
   let secret_key_serialized:t_Array u8 v_PRIVATE_KEY_SIZE =
-    Libcrux.Kem.Kyber.Ind_cpa.serialize_secret_key #p v_PRIVATE_KEY_SIZE
-      (Rust_primitives.unsize (Libcrux.Kem.Kyber.Types.impl_30__as_slice v_CPA_PRIVATE_KEY_SIZE
-              ind_cpa_private_key
-            <:
-            t_Array u8 v_CPA_PRIVATE_KEY_SIZE)
-        <:
-        t_Slice u8)
-      (Rust_primitives.unsize (Libcrux.Kem.Kyber.Types.impl_24__as_slice v_PUBLIC_KEY_SIZE
-              public_key
-            <:
-            t_Array u8 v_PUBLIC_KEY_SIZE)
-        <:
-        t_Slice u8)
+    serialize_kem_secret_key #p v_PRIVATE_KEY_SIZE
+      (Rust_primitives.unsize ind_cpa_private_key <: t_Slice u8)
+      (Rust_primitives.unsize public_key <: t_Slice u8)
       implicit_rejection_value
   in
   let res = 
   match sampling_a_error with
-  | Core.Option.Option_Some error -> (
+  | Core.Option.Option_Some error ->
     Core.Result.Result_Err error
     <:
     Core.Result.t_Result
       (Libcrux.Kem.Kyber.Types.t_KyberKeyPair v_PRIVATE_KEY_SIZE v_PUBLIC_KEY_SIZE)
-      Libcrux.Kem.Kyber.Types.t_Error)
-  | _ -> (
+      Libcrux.Kem.Kyber.Types.t_Error
+  | _ ->
     let (private_key: Libcrux.Kem.Kyber.Types.t_KyberPrivateKey v_PRIVATE_KEY_SIZE):Libcrux.Kem.Kyber.Types.t_KyberPrivateKey
     v_PRIVATE_KEY_SIZE =
       Core.Convert.f_from secret_key_serialized
     in
     Core.Result.Result_Ok
-    (Libcrux.Kem.Kyber.Types.impl__from v_PRIVATE_KEY_SIZE v_PUBLIC_KEY_SIZE private_key public_key)
+    (Libcrux.Kem.Kyber.Types.impl__from v_PRIVATE_KEY_SIZE
+        v_PUBLIC_KEY_SIZE
+        private_key
+        (Core.Convert.f_into public_key
+          <:
+          Libcrux.Kem.Kyber.Types.t_KyberPublicKey v_PUBLIC_KEY_SIZE))
     <:
     Core.Result.t_Result
       (Libcrux.Kem.Kyber.Types.t_KyberKeyPair v_PRIVATE_KEY_SIZE v_PUBLIC_KEY_SIZE)
-      Libcrux.Kem.Kyber.Types.t_Error)
-  in 
-  res
+      Libcrux.Kem.Kyber.Types.t_Error
+   in
+   res
